Inductive tr_expression + fix spec

src/SimplExprproof.v
@@ -25,8 +25,8 @@ Notation "a ! b" := (get b a) (at level 1).
 (** ** Relational specification of the translation. *)
 
 Definition match_prog (p: Csyntax.program) (tp: Clight.program) :=
-    match_program (fun ctx f tf => tr_fundef f tf) eq p tp
- /\ prog_types tp = prog_types p.
+  match_program (fun ctx f tf => tr_fundef f tf) eq p tp
+  /\ prog_types tp = prog_types p.
 
 Lemma transf_program_match:
   forall p tp, transl_program p = OK tp -> match_prog p tp.
@@ -41,347 +41,349 @@ Qed.
 
 Section PRESERVATION.
 
-Variable prog: Csyntax.program.
-Variable tprog: Clight.program.
-Hypothesis TRANSL: match_prog prog tprog.
+  Variable prog: Csyntax.program.
+  Variable tprog: Clight.program.
+  Hypothesis TRANSL: match_prog prog tprog.
 
-Let ge := Csem.globalenv prog.
-Let tge := Clight.globalenv tprog.
+  Let ge := Csem.globalenv prog.
+  Let tge := Clight.globalenv tprog.
 
-(** Invariance properties. *)
+  (** Invariance properties. *)
 
-Lemma comp_env_preserved:
-  Clight.genv_cenv tge = Csem.genv_cenv ge.
-Proof.
-  simpl. destruct TRANSL. generalize (prog_comp_env_eq tprog) (prog_comp_env_eq prog). 
-  congruence.
-Qed.
+  Lemma comp_env_preserved:
+    Clight.genv_cenv tge = Csem.genv_cenv ge.
+  Proof.
+    simpl. destruct TRANSL. generalize (prog_comp_env_eq tprog) (prog_comp_env_eq prog). 
+    congruence.
+  Qed.
 
-Lemma symbols_preserved:
-  forall (s: ident), Genv.find_symbol tge s = Genv.find_symbol ge s.
-Proof (Genv.find_symbol_match (proj1 TRANSL)).
+  Lemma symbols_preserved:
+    forall (s: ident), Genv.find_symbol tge s = Genv.find_symbol ge s.
+  Proof (Genv.find_symbol_match (proj1 TRANSL)).
 
-Lemma senv_preserved:
-  Senv.equiv ge tge.
-Proof (Genv.senv_match (proj1 TRANSL)).
+  Lemma senv_preserved:
+    Senv.equiv ge tge.
+  Proof (Genv.senv_match (proj1 TRANSL)).
 
-Lemma function_ptr_translated:
-  forall b f,
-  Genv.find_funct_ptr ge b = Some f ->
-  exists tf,
-  Genv.find_funct_ptr tge b = Some tf /\ tr_fundef f tf.
-Proof.
-  intros.
-  edestruct (Genv.find_funct_ptr_match (proj1 TRANSL)) as (ctx & tf & A & B & C); eauto.
-Qed.
+  Lemma function_ptr_translated:
+    forall b f,
+      Genv.find_funct_ptr ge b = Some f ->
+      exists tf,
+        Genv.find_funct_ptr tge b = Some tf /\ tr_fundef f tf.
+  Proof.
+    intros.
+    edestruct (Genv.find_funct_ptr_match (proj1 TRANSL)) as (ctx & tf & A & B & C); eauto.
+  Qed.
 
-Lemma functions_translated:
-  forall v f,
-  Genv.find_funct ge v = Some f ->
-  exists tf,
-  Genv.find_funct tge v = Some tf /\ tr_fundef f tf.
-Proof.
-  intros.
-  edestruct (Genv.find_funct_match (proj1 TRANSL)) as (ctx & tf & A & B & C); eauto.
-Qed.
+  Lemma functions_translated:
+    forall v f,
+      Genv.find_funct ge v = Some f ->
+      exists tf,
+        Genv.find_funct tge v = Some tf /\ tr_fundef f tf.
+  Proof.
+    intros.
+    edestruct (Genv.find_funct_match (proj1 TRANSL)) as (ctx & tf & A & B & C); eauto.
+  Qed.
 
-Lemma type_of_fundef_preserved:
-  forall f tf, tr_fundef f tf ->
-  type_of_fundef tf = Csyntax.type_of_fundef f.
-Proof.
-  intros. inv H.
-  inv H0; simpl. unfold type_of_function, Csyntax.type_of_function. congruence.
-  auto.
-Qed.
+  Lemma type_of_fundef_preserved:
+    forall f tf, tr_fundef f tf ->
+            type_of_fundef tf = Csyntax.type_of_fundef f.
+  Proof.
+    intros. inv H.
+    inv H0; simpl. unfold type_of_function, Csyntax.type_of_function. congruence.
+    auto.
+  Qed.
 
-Lemma function_return_preserved:
-  forall f tf, tr_function f tf ->
-  fn_return tf = Csyntax.fn_return f.
-Proof.
-  intros. inv H; auto.
-Qed.
+  Lemma function_return_preserved:
+    forall f tf, tr_function f tf ->
+            fn_return tf = Csyntax.fn_return f.
+  Proof.
+    intros. inv H; auto.
+  Qed.
 
-(** Properties of smart constructors. *)
+  (** Properties of smart constructors. *)
 
-Lemma eval_Ederef':
-  forall ge e le m a t l ofs,
-  eval_expr ge e le m a (Vptr l ofs) ->
-  eval_lvalue ge e le m (Ederef' a t) l ofs.
-Proof.
-  intros. unfold Ederef'; destruct a; auto using eval_Ederef.
-  destruct (type_eq t0 (typeof a)); auto using eval_Ederef.
-  inv H.
-- auto. 
-- inv H0.
-Qed.
+  Lemma eval_Ederef':
+    forall ge e le m a t l ofs,
+      eval_expr ge e le m a (Vptr l ofs) ->
+      eval_lvalue ge e le m (Ederef' a t) l ofs.
+  Proof.
+    intros. unfold Ederef'; destruct a; auto using eval_Ederef.
+    destruct (type_eq t0 (typeof a)); auto using eval_Ederef.
+    inv H.
+    - auto. 
+    - inv H0.
+  Qed.
 
-Lemma typeof_Ederef':
-  forall a t, typeof (Ederef' a t) = t.
-Proof.
-  unfold Ederef'; intros; destruct a; auto. destruct (type_eq t0 (typeof a)); auto. 
-Qed.
+  Lemma typeof_Ederef':
+    forall a t, typeof (Ederef' a t) = t.
+  Proof.
+    unfold Ederef'; intros; destruct a; auto. destruct (type_eq t0 (typeof a)); auto. 
+  Qed.
 
-Lemma eval_Eaddrof':
-  forall ge e le m a t l ofs,
-  eval_lvalue ge e le m a l ofs ->
-  eval_expr ge e le m (Eaddrof' a t) (Vptr l ofs).
-Proof.
-  intros. unfold Eaddrof'; destruct a; auto using eval_Eaddrof.
-  destruct (type_eq t0 (typeof a)); auto using eval_Eaddrof.
-  inv H; auto.
-Qed.
+  Lemma eval_Eaddrof':
+    forall ge e le m a t l ofs,
+      eval_lvalue ge e le m a l ofs ->
+      eval_expr ge e le m (Eaddrof' a t) (Vptr l ofs).
+  Proof.
+    intros. unfold Eaddrof'; destruct a; auto using eval_Eaddrof.
+    destruct (type_eq t0 (typeof a)); auto using eval_Eaddrof.
+    inv H; auto.
+  Qed.
 
-Lemma typeof_Eaddrof':
-  forall a t, typeof (Eaddrof' a t) = t.
-Proof.
-  unfold Eaddrof'; intros; destruct a; auto. destruct (type_eq t0 (typeof a)); auto. 
-Qed.
+  Lemma typeof_Eaddrof':
+    forall a t, typeof (Eaddrof' a t) = t.
+  Proof.
+    unfold Eaddrof'; intros; destruct a; auto. destruct (type_eq t0 (typeof a)); auto. 
+  Qed.
 
-(** Translation of simple expressions. *)
+  (** Translation of simple expressions. *)
 
-Lemma pair_equal_spec :
-  forall (A B : Type) (a1 a2 : A) (b1 b2 : B),
-    (a1, b1) = (a2, b2) <-> a1 = a2 /\ b1 = b2.
-Proof.
-  intros. split; intro H; inversion H; subst; eauto.
-Qed.
+  Lemma pair_equal_spec :
+    forall (A B : Type) (a1 a2 : A) (b1 b2 : B),
+      (a1, b1) = (a2, b2) <-> a1 = a2 /\ b1 = b2.
+  Proof.
+    intros. split; intro H; inversion H; subst; eauto.
+  Qed.
 
-Import adequacy.
+  Import adequacy.
 
-Lemma tr_simple_nil:
-  (forall r dst sl le a, tr_expr le dst r (sl,a) -∗
-   ⌜ dst = For_val \/ dst = For_effects ⌝ -∗ ⌜ simple r = true ⌝ -∗ ⌜sl = nil ⌝)
-/\(forall rl le sl al, tr_exprlist le rl (sl,al) -∗
-   ⌜ simplelist rl = true ⌝ -∗ ⌜ sl = nil ⌝).
-Proof.
-  assert (A: forall dst a, dst = For_val \/ dst = For_effects -> final dst a = nil).
-  intros. destruct H; subst dst; auto.
-  apply tr_expr_exprlist; intros; simpl in *; try discriminate; auto.
-  - destruct dst.
-    + iIntros "[% [% %]]". iPureIntro. intros; auto.
-    + iIntros. iPureIntro. intros; auto.
-    + iIntros "[% [% %]]". iPureIntro. intros. destruct H2; discriminate.
-  - iIntros "[_ %]". iPureIntro. intros. inversion H. destruct dst; auto.
-  - iIntros "HA". iDestruct "HA" as (sla2) "[HA [HB %]]".
-    rewrite (surjective_pairing sla2). iIntros.
-    iDestruct (H with "[HA]") as "HC". iApply "HA".
-    destruct dst.
-    + iDestruct ("HC" $! a0 a1) as "HA". simpl in *. inversion H0. rewrite app_nil_r. iApply "HA". 
-    + iDestruct ("HC" with "[]") as "HA"; eauto. inversion H0. rewrite app_nil_r.
-      iApply ("HA" $! a1).
-    + destruct a0; discriminate.
-  - iIntros "HA % %". iDestruct "HA" as (sla2 sl3) "[HA [HB [HC %]]]".
-    rewrite (surjective_pairing sla2).
-    iDestruct (H with "HA") as "HD".
-    apply andb_true_iff in a1 as (P0&P1).
-    unfold tr_rvalof. apply negb_true_iff in P1. rewrite P1.
-    iDestruct "HB" as "%". inversion H1; subst. destruct dst; simpl in *; try rewrite app_nil_r.
-    + iApply ("HD" $! a0 P0).
-    + iApply "HD"; eauto.
-    + destruct a0; discriminate.
-  - iIntros "HA % %". iDestruct "HA" as (sla2) "[HA [HB %]]".
-    rewrite (surjective_pairing sla2).
-    iDestruct (H with "HA") as "HD".
-    inversion H0.
-    destruct dst; simpl in *; try (rewrite app_nil_r; iApply "HD";eauto); destruct a0; discriminate.
-  - iIntros "HA % %". iDestruct "HA" as (sla2) "[HA [HB %]]".
-    rewrite (surjective_pairing sla2).
-    iDestruct (H with "HA") as "HD".
-    inversion H0.
-    destruct dst; simpl in *; try (rewrite app_nil_r; iApply "HD";eauto); destruct a0; discriminate.
-  - iIntros "HA % %". iDestruct "HA" as (sla2) "[HA [HB %]]".
-    rewrite (surjective_pairing sla2).
-    iDestruct (H with "HA") as "HD".
-    inversion H0.
-    destruct dst; simpl in *; try (rewrite app_nil_r; iApply "HD";eauto); destruct a0; discriminate.
-  - iIntros "HA % %". iDestruct "HA" as (sla2 sl3) "[HA [HB [HC %]]]".
-    rewrite (surjective_pairing sla2).
-    iDestruct (H with "HA") as "HD".
-    rewrite (surjective_pairing sl3).
-    iDestruct (H0 with "HB") as "HB".
-    apply andb_true_iff in a1 as (P0&P1).
-    inversion H1.
-    iDestruct ("HD" with "[]") as "%"; eauto.
-    iDestruct ("HB" with "[]") as "%"; eauto.
-    iPureIntro. rewrite (H2 P0). rewrite (H5 P1).
-    destruct a0; subst; auto.
-  - iIntros "HA % %". iDestruct "HA" as (sla2) "[HA [HB %]]".
-    rewrite (surjective_pairing sla2).
-    iDestruct (H with "HA") as "HD".
-    inversion H0.
-    destruct dst; simpl in *; try (rewrite app_nil_r; iApply "HD";eauto); destruct a0; discriminate.
-  - iIntros "[HA %] % %". inversion H.
-    destruct dst; eauto.
-  - iIntros "[HA %] % %". inversion H.
-    destruct dst; eauto.
-  - iIntros "% %". inversion a; eauto.
-  - iIntros "HA %". iDestruct "HA" as (sla2 slal3) "[HA [HB %]]".
-    rewrite (surjective_pairing sla2).
-    iDestruct (H with "[HA]") as "HC". iApply "HA".
-    rewrite (surjective_pairing slal3).
-    iDestruct (H0 with "[HB]") as "HA". iApply "HB".
-    iDestruct ("HC" with "[]") as "%"; eauto.
-    apply andb_true_iff in a as (P0&P1).
-    iDestruct ("HA" with "[]") as "%"; eauto.
-    iPureIntro. inversion H1. rewrite (H2 P0). rewrite H3. eauto.
-Qed.
+  Lemma tr_simple_nil:
+    (forall r dst sl le a, tr_expr le dst r (sl,a) -∗
+                                   ⌜ dst = For_val \/ dst = For_effects ⌝ -∗ ⌜ simple r = true ⌝ -∗ ⌜sl = nil ⌝)
+    /\(forall rl le sl al, tr_exprlist le rl (sl,al) -∗
+                                       ⌜ simplelist rl = true ⌝ -∗ ⌜ sl = nil ⌝).
+  Proof.
+    assert (A: forall dst a, dst = For_val \/ dst = For_effects -> final dst a = nil).
+    intros. destruct H; subst dst; auto.
+    apply tr_expr_exprlist; intros; simpl in *; try discriminate; auto.
+    - destruct dst; eauto.
+      + iIntros "[_ [HA [% %]]] _ _". eauto.
+      + iIntros "[_ %] % _". eauto.
+      + iIntros "[_ HA] % _". destruct a0; discriminate.
+    - iIntros "[_ [_ %]]". iPureIntro. intros. inversion H. destruct dst; auto.
+    - iIntros "[_ HA]". iDestruct "HA" as (sla2) "[HA [HB %]]".
+      rewrite (surjective_pairing sla2). iIntros.
+      iDestruct (H with "[HA]") as "HC". iApply "HA".
+      destruct dst.
+      + iDestruct ("HC" $! a0 a1) as "HA". simpl in *. inversion H0. rewrite app_nil_r. iApply "HA". 
+      + iDestruct ("HC" with "[]") as "HA"; eauto. inversion H0. rewrite app_nil_r.
+        iApply ("HA" $! a1).
+      + destruct a0; discriminate.
+    - iIntros "[_ HA] % %". iDestruct "HA" as (sla2 sl3) "[HA [HB [HC %]]]".
+      rewrite (surjective_pairing sla2).
+      iDestruct (H with "HA") as "HD".
+      apply andb_true_iff in a1 as (P0&P1).
+      unfold tr_rvalof. apply negb_true_iff in P1. rewrite P1.
+      iDestruct "HB" as "%". inversion H1; subst. destruct dst; simpl in *; try rewrite app_nil_r.
+      + iApply ("HD" $! a0 P0).
+      + iApply "HD"; eauto.
+      + destruct a0; discriminate.
+    - iIntros "[_ HA] % %". iDestruct "HA" as (sla2) "[HA [HB %]]".
+      rewrite (surjective_pairing sla2).
+      iDestruct (H with "HA") as "HD".
+      inversion H0.
+      destruct dst; simpl in *; try (rewrite app_nil_r; iApply "HD";eauto); destruct a0; discriminate.
+    - iIntros "[_ HA] % %". iDestruct "HA" as (sla2) "[HA [HB %]]".
+      rewrite (surjective_pairing sla2).
+      iDestruct (H with "HA") as "HD".
+      inversion H0.
+      destruct dst; simpl in *; try (rewrite app_nil_r; iApply "HD";eauto); destruct a0; discriminate.
+    - iIntros "[_ HA] % %". iDestruct "HA" as (sla2) "[HA [HB %]]".
+      rewrite (surjective_pairing sla2).
+      iDestruct (H with "HA") as "HD".
+      inversion H0.
+      destruct dst; simpl in *; try (rewrite app_nil_r; iApply "HD";eauto); destruct a0; discriminate.
+    - iIntros "[_ HA] % %". iDestruct "HA" as (sla2 sl3) "[HA [HB [HC %]]]".
+      rewrite (surjective_pairing sla2).
+      iDestruct (H with "HA") as "HD".
+      rewrite (surjective_pairing sl3).
+      iDestruct (H0 with "HB") as "HB".
+      apply andb_true_iff in a1 as (P0&P1).
+      inversion H1.
+      iDestruct ("HD" with "[]") as "%"; eauto.
+      iDestruct ("HB" with "[]") as "%"; eauto.
+      iPureIntro. rewrite (H2 P0). rewrite (H5 P1).
+      destruct a0; subst; auto.
+    - iIntros "[_ HA] % %". iDestruct "HA" as (sla2) "[HA [HB %]]".
+      rewrite (surjective_pairing sla2).
+      iDestruct (H with "HA") as "HD".
+      inversion H0.
+      destruct dst; simpl in *; try (rewrite app_nil_r; iApply "HD";eauto); destruct a0; discriminate.
+    - iIntros "[_ [HA %]] % %". inversion H.
+      destruct dst; eauto.
+    - iIntros "[_ [HA %]] % %". inversion H.
+      destruct dst; eauto.
+    - iIntros "[_ %] %". inversion H.
+    - iIntros "[_ %] %". inversion H; eauto.
+    - iIntros "[_ HA] %". iDestruct "HA" as (sla2 slal3) "[HA [HB %]]".
+      rewrite (surjective_pairing sla2).
+      iDestruct (H with "[HA]") as "HC". iApply "HA".
+      rewrite (surjective_pairing slal3).
+      iDestruct (H0 with "[HB]") as "HA". iApply "HB".
+      iDestruct ("HC" with "[]") as "%"; eauto.
+      apply andb_true_iff in a as (P0&P1).
+      iDestruct ("HA" with "[]") as "%"; eauto.
+      iPureIntro. inversion H1. rewrite (H2 P0). rewrite H3. eauto.
+  Qed.
 
-Lemma tr_simple_expr_nil:
-  (forall r dst sl le a, tr_expr le dst r (sl,a) -∗
-   ⌜ dst = For_val \/ dst = For_effects ⌝ -∗ ⌜ simple r = true ⌝ -∗ ⌜sl = nil ⌝).
-Proof (proj1 tr_simple_nil).
+  Lemma tr_simple_expr_nil:
+    (forall r dst sl le a, tr_expr le dst r (sl,a) -∗
+                                   ⌜ dst = For_val \/ dst = For_effects ⌝ -∗ ⌜ simple r = true ⌝ -∗ ⌜sl = nil ⌝).
+  Proof (proj1 tr_simple_nil).
 
-Lemma tr_simple_exprlist_nil:
-  (forall rl le sl al, tr_exprlist le rl (sl,al) -∗
-   ⌜ simplelist rl = true ⌝ -∗ ⌜ sl = nil ⌝).
-Proof (proj2 tr_simple_nil).
+  Lemma tr_simple_exprlist_nil:
+    (forall rl le sl al, tr_exprlist le rl (sl,al) -∗
+                                     ⌜ simplelist rl = true ⌝ -∗ ⌜ sl = nil ⌝).
+  Proof (proj2 tr_simple_nil).
 
-(** Translation of [deref_loc] and [assign_loc] operations. *)
+  (** Translation of [deref_loc] and [assign_loc] operations. *)
 
-Remark deref_loc_translated:
-  forall ty m b ofs t v,
-  Csem.deref_loc ge ty m b ofs t v ->
-  match chunk_for_volatile_type ty with
-  | None => t = E0 /\ Clight.deref_loc ty m b ofs v
-  | Some chunk => volatile_load tge chunk m b ofs t v
-  end.
-Proof.
-  intros. unfold chunk_for_volatile_type. inv H.
-  (* By_value, not volatile *)
-  rewrite H1. split; auto. eapply deref_loc_value; eauto.
-  (* By_value, volatile *)
-  rewrite H0; rewrite H1. eapply volatile_load_preserved with (ge1 := ge); auto. apply senv_preserved.
-  (* By reference *)
-  rewrite H0. destruct (type_is_volatile ty); split; auto; eapply deref_loc_reference; eauto.
-  (* By copy *)
-  rewrite H0. destruct (type_is_volatile ty); split; auto; eapply deref_loc_copy; eauto.
-Qed.
+  Remark deref_loc_translated:
+    forall ty m b ofs t v,
+      Csem.deref_loc ge ty m b ofs t v ->
+      match chunk_for_volatile_type ty with
+      | None => t = E0 /\ Clight.deref_loc ty m b ofs v
+      | Some chunk => volatile_load tge chunk m b ofs t v
+      end.
+  Proof.
+    intros. unfold chunk_for_volatile_type. inv H.
+    (* By_value, not volatile *)
+    rewrite H1. split; auto. eapply deref_loc_value; eauto.
+    (* By_value, volatile *)
+    rewrite H0; rewrite H1. eapply volatile_load_preserved with (ge1 := ge); auto. apply senv_preserved.
+    (* By reference *)
+    rewrite H0. destruct (type_is_volatile ty); split; auto; eapply deref_loc_reference; eauto.
+    (* By copy *)
+    rewrite H0. destruct (type_is_volatile ty); split; auto; eapply deref_loc_copy; eauto.
+  Qed.
 
-Remark assign_loc_translated:
-  forall ty m b ofs v t m',
-  Csem.assign_loc ge ty m b ofs v t m' ->
-  match chunk_for_volatile_type ty with
-  | None => t = E0 /\ Clight.assign_loc tge ty m b ofs v m'
-  | Some chunk => volatile_store tge chunk m b ofs v t m'
-  end.
-Proof.
-  intros. unfold chunk_for_volatile_type. inv H.
-  (* By_value, not volatile *)
-  rewrite H1. split; auto. eapply assign_loc_value; eauto.
-  (* By_value, volatile *)
-  rewrite H0; rewrite H1. eapply volatile_store_preserved with (ge1 := ge); auto. apply senv_preserved.
-  (* By copy *)
-  rewrite H0. rewrite <- comp_env_preserved in *.
-  destruct (type_is_volatile ty); split; auto; eapply assign_loc_copy; eauto.
-Qed.
+  Remark assign_loc_translated:
+    forall ty m b ofs v t m',
+      Csem.assign_loc ge ty m b ofs v t m' ->
+      match chunk_for_volatile_type ty with
+      | None => t = E0 /\ Clight.assign_loc tge ty m b ofs v m'
+      | Some chunk => volatile_store tge chunk m b ofs v t m'
+      end.
+  Proof.
+    intros. unfold chunk_for_volatile_type. inv H.
+    (* By_value, not volatile *)
+    rewrite H1. split; auto. eapply assign_loc_value; eauto.
+    (* By_value, volatile *)
+    rewrite H0; rewrite H1. eapply volatile_store_preserved with (ge1 := ge); auto. apply senv_preserved.
+    (* By copy *)
+    rewrite H0. rewrite <- comp_env_preserved in *.
+    destruct (type_is_volatile ty); split; auto; eapply assign_loc_copy; eauto.
+  Qed.
 
-(** Evaluation of simple expressions and of their translation *)
+  (** Evaluation of simple expressions and of their translation *)
 
-Lemma tr_simple:
- forall e m,
- (forall r v,
-  eval_simple_rvalue ge e m r v ->
-  forall le dst sl a,
-  (tr_expr le dst r (sl,a)) -∗
-  ⌜ match dst with
-    | For_val => sl = nil /\ Csyntax.typeof r = typeof a /\ eval_expr tge e le m a v
-  | For_effects => sl = nil
-  | For_set sd =>
-      exists b, sl = do_set sd b
-             /\ Csyntax.typeof r = typeof b
-             /\ eval_expr tge e le m b v
-  end⌝)
-/\
- (forall l b ofs,
-  eval_simple_lvalue ge e m l b ofs ->
-  forall le sl a, tr_expr le For_val l (sl,a) -∗                                               
-  ⌜ sl = nil /\ Csyntax.typeof l = typeof a /\ eval_lvalue tge e le m a b ofs ⌝).
-Proof.
-Opaque makeif.
-intros e m.
-apply (eval_simple_rvalue_lvalue_ind ge e m); intros; simpl.
-(* value *)
-- destruct dst; simpl in *; iIntros "%".
-  + destruct a0 as (P0&P1&P2). iPureIntro. repeat split; auto. 
-  + iPureIntro. assumption.
-  + iExists a. destruct a0 as (P0&P1&P2). iPureIntro. split; auto.
-(* rvalof *)
-- destruct dst; subst; simpl in *.
-  + iIntros "HA". iDestruct "HA" as (sla2 sl3) "[HA [HB [_ %]]]".
-    rewrite (surjective_pairing sla2).
-    iDestruct (H0 with "HA") as "[% [% %]]".
-    unfold tr_rvalof. rewrite H2. iDestruct "HB" as "%". inversion H7; subst.
-    iPureIntro. repeat split; auto. do 2 rewrite app_nil_r. apply H4.
-    eapply eval_Elvalue; eauto.
-    exploit deref_loc_translated; eauto. unfold chunk_for_volatile_type; rewrite H2.
-    intros (P0&P1). rewrite <- H5. assumption.
-  + iIntros "HA". iDestruct "HA" as (sla2 sl3) "[HA [HB [_ %]]]".
-    rewrite (surjective_pairing sla2).
-    iDestruct (H0 with "HA") as "[% [% %]]".
-    unfold tr_rvalof. rewrite H2. iDestruct "HB" as "%". inversion H7; subst.
-    iPureIntro. do 2 rewrite app_nil_r. apply H4.
-  + iIntros "HA". iDestruct "HA" as (sla2 sl3) "[HA [HB [_ %]]]". iExists a.
-    rewrite (surjective_pairing sla2).
-    iDestruct (H0 with "HA") as "[% [% %]]".
-    unfold tr_rvalof. rewrite H2. iDestruct "HB" as "%". inversion H7; subst.
-    iPureIntro. repeat split; auto. rewrite H4. do 2 rewrite app_nil_l. reflexivity.
-    eapply eval_Elvalue; eauto.
-    exploit deref_loc_translated; eauto. unfold chunk_for_volatile_type; rewrite H2.
-    intros (P0&P1). rewrite <- H5. apply P1.
-- iIntros "HA". iDestruct "HA" as (sla2) "[HA [HB %]]". rewrite (surjective_pairing sla2).
-  iDestruct (H0 with "HA") as "[% [% %]]". inversion H1.
-  destruct dst; simpl in *; subst.
-  + iPureIntro. repeat split; auto.
-    * rewrite app_nil_r. apply H2.
-    * rewrite (typeof_Eaddrof' sla2.2 ty). reflexivity.
-    * apply eval_Eaddrof'; auto.
-  + iPureIntro. rewrite app_nil_r. apply H2.
-  + iExists (Eaddrof' sla2.2 ty). iPureIntro. repeat split.
-    * rewrite H2. rewrite app_nil_l. reflexivity.
-    * rewrite (typeof_Eaddrof' sla2.2 ty). reflexivity.
-    * apply eval_Eaddrof'; auto.
-- iIntros "HA". iDestruct "HA" as (sla2) "[HA [HB %]]". rewrite (surjective_pairing sla2).
-  iDestruct (H0 with "HA") as "[% [% %]]". inversion H2.
-  destruct dst; simpl in *; subst.
-  + iPureIntro. repeat split; auto.
-    * rewrite app_nil_r. apply H3.
-    * rewrite H4 in H1. econstructor; eauto.
-  + iPureIntro. rewrite app_nil_r. apply H3.
-  + iExists (Eunop op0 sla2.2 ty). iPureIntro. repeat split.
-    * rewrite H3. rewrite app_nil_l. reflexivity.
-    * rewrite H4 in H1. econstructor; eauto.
-- iIntros "HA". iDestruct "HA" as (sla2 sla3) "[HA [HB [HC %]]]". rewrite (surjective_pairing sla2).
-  iDestruct (H0 with "HA") as "[% [% %]]". rewrite (surjective_pairing sla3).
-  iDestruct (H2 with "HB") as "[% [% %]]". inversion H4.
-  destruct dst; simpl in *; subst; rewrite H5 H8; try iExists (Ebinop op0 sla2.2 sla3.2 ty);
-    do 2 rewrite app_nil_l; iPureIntro; repeat split; auto; econstructor; eauto; rewrite <- H6;
-      auto; rewrite <- H9; rewrite comp_env_preserved; apply H3.
-- iIntros "HA". iDestruct "HA" as (sla2)  "[HA [HB %]]". rewrite (surjective_pairing sla2).
-  iDestruct (H0 with "HA") as "[% [% %]]". inversion H2.
-  destruct dst; simpl in *; subst; rewrite H3; try iExists (Ecast sla2.2 ty); iPureIntro;
-    rewrite app_nil_l; repeat split; auto; econstructor; eauto; rewrite <- H4; auto.
-- iIntros "[HA %]". inversion H.
-  destruct dst; simpl in *; subst; try iExists (Esizeof ty1 ty); iPureIntro; repeat split; eauto;
-    pose (P := comp_env_preserved); simpl in P; rewrite <- P; apply eval_Esizeof.
-- iIntros "[HA %]". inversion H.
-  destruct dst; simpl in *; subst; try iExists (Ealignof ty1 ty); iPureIntro; repeat split; eauto;
-    pose (P := comp_env_preserved); simpl in P; rewrite <- P; constructor.
-- iIntros. contradiction a0.
-- iIntros "[_ %]". inversion H0. iPureIntro. repeat split; auto. constructor. apply H.
-- iIntros "[_ %]". inversion H1. iPureIntro. repeat split; auto.
-  apply eval_Evar_global; auto.
-  rewrite symbols_preserved; auto.
-- iIntros "HA". iDestruct "HA" as (sla2)  "[HA [HB %]]". rewrite (surjective_pairing sla2).
-  iDestruct (H0 with "HA") as "[% [% %]]". inversion H1. iPureIntro. subst. repeat split.
-  rewrite app_nil_r. apply H2. rewrite typeof_Ederef'; auto. apply eval_Ederef'; auto. 
-- iIntros "HA". iDestruct "HA" as (sla2)  "[HA [HB %]]". rewrite (surjective_pairing sla2).
-  iDestruct (H0 with "HA") as "[% [% %]]". inversion H4. subst. iPureIntro. repeat split.
-  rewrite app_nil_r. apply H5. rewrite <- comp_env_preserved in *. rewrite H6 in H1.
-  eapply eval_Efield_struct; eauto.
-- iIntros "HA". iDestruct "HA" as (sla2)  "[HA [HB %]]". rewrite (surjective_pairing sla2).
-  iDestruct (H0 with "HA") as "[% [% %]]". inversion H3. subst. iPureIntro. repeat split.
-  rewrite app_nil_r. apply H4. rewrite <- comp_env_preserved in *. rewrite H5 in H1.
-  eapply eval_Efield_union; eauto.
+  Lemma tr_simple:
+    forall e m,
+      (forall r v,
+          eval_simple_rvalue ge e m r v ->
+          forall le dst sl a,
+            (tr_expr le dst r (sl,a)) -∗
+                                      ⌜ match dst with
+                                        | For_val => sl = nil /\ Csyntax.typeof r = typeof a /\ eval_expr tge e le m a v
+                                        | For_effects => sl = nil
+                                        | For_set sd =>
+                                          exists b, sl = do_set sd b
+                                                    /\ Csyntax.typeof r = typeof b
+                                                    /\ eval_expr tge e le m b v
+                                        end⌝)
+      /\
+      (forall l b ofs,
+          eval_simple_lvalue ge e m l b ofs ->
+          forall le sl a, tr_expr le For_val l (sl,a) -∗                                               
+                                  ⌜ sl = nil /\ Csyntax.typeof l = typeof a /\ eval_lvalue tge e le m a b ofs ⌝).
+  Proof.
+    Opaque makeif.
+    intros e m.
+    apply (eval_simple_rvalue_lvalue_ind ge e m); intros; simpl.
+    (* value *)
+    - destruct dst; simpl in *; auto.
+      + iIntros "[_ [HA [% %]]]". repeat (iSplit; auto). iApply "HA". eauto.
+      + iIntros "[_ HA]"; auto. 
+      + iIntros "[_ HA]". iDestruct "HA" as (a0) "[HA [% %]]". subst. iExists a0. repeat iSplit; eauto.
+        iApply "HA". auto.
+    (* rvalof *)
+    - destruct dst; subst; simpl in *.
+      + iIntros "[_ HA]". iDestruct "HA" as (sla2 sl3) "[HA [HB [_ %]]]".
+        rewrite (surjective_pairing sla2).
+        iDestruct (H0 with "HA") as "[% [% %]]".
+        unfold tr_rvalof. rewrite H2. iDestruct "HB" as "%". inversion H7; subst.
+        iPureIntro. repeat split; auto. do 2 rewrite app_nil_r. apply H4.
+        eapply eval_Elvalue; eauto.
+        exploit deref_loc_translated; eauto. unfold chunk_for_volatile_type; rewrite H2.
+        intros (P0&P1). rewrite <- H5. assumption.
+      + iIntros "[_ HA]". iDestruct "HA" as (sla2 sl3) "[HA [HB [_ %]]]".
+        rewrite (surjective_pairing sla2).
+        iDestruct (H0 with "HA") as "[% [% %]]".
+        unfold tr_rvalof. rewrite H2. iDestruct "HB" as "%". inversion H7; subst.
+        iPureIntro. do 2 rewrite app_nil_r. apply H4.
+      + iIntros "[_ HA]". iDestruct "HA" as (sla2 sl3) "[HA [HB [_ %]]]". iExists a.
+        rewrite (surjective_pairing sla2).
+        iDestruct (H0 with "HA") as "[% [% %]]".
+        unfold tr_rvalof. rewrite H2. iDestruct "HB" as "%". inversion H7; subst.
+        iPureIntro. repeat split; auto. rewrite H4. do 2 rewrite app_nil_l. reflexivity.
+        eapply eval_Elvalue; eauto.
+        exploit deref_loc_translated; eauto. unfold chunk_for_volatile_type; rewrite H2.
+        intros (P0&P1). rewrite <- H5. apply P1.
+    - iIntros "[_ HA]". iDestruct "HA" as (sla2) "[HA [HB %]]". rewrite (surjective_pairing sla2).
+      iDestruct (H0 with "HA") as "[% [% %]]". inversion H1.
+      destruct dst; simpl in *; subst.
+      + iPureIntro. repeat split; auto.
+        * rewrite app_nil_r. apply H2.
+        * rewrite (typeof_Eaddrof' sla2.2 ty). reflexivity.
+        * apply eval_Eaddrof'; auto.
+      + iPureIntro. rewrite app_nil_r. apply H2.
+      + iExists (Eaddrof' sla2.2 ty). iPureIntro. repeat split.
+        * rewrite H2. rewrite app_nil_l. reflexivity.
+        * rewrite (typeof_Eaddrof' sla2.2 ty). reflexivity.
+        * apply eval_Eaddrof'; auto.
+    - iIntros "[_ HA]". iDestruct "HA" as (sla2) "[HA [HB %]]". rewrite (surjective_pairing sla2).
+      iDestruct (H0 with "HA") as "[% [% %]]". inversion H2.
+      destruct dst; simpl in *; subst.
+      + iPureIntro. repeat split; auto.
+        * rewrite app_nil_r. apply H3.
+        * rewrite H4 in H1. econstructor; eauto.
+      + iPureIntro. rewrite app_nil_r. apply H3.
+      + iExists (Eunop op0 sla2.2 ty). iPureIntro. repeat split.
+        * rewrite H3. rewrite app_nil_l. reflexivity.
+        * rewrite H4 in H1. econstructor; eauto.
+    - iIntros "[_ HA]". iDestruct "HA" as (sla2 sla3) "[HA [HB [HC %]]]". rewrite (surjective_pairing sla2).
+      iDestruct (H0 with "HA") as "[% [% %]]". rewrite (surjective_pairing sla3).
+      iDestruct (H2 with "HB") as "[% [% %]]". inversion H4.
+      destruct dst; simpl in *; subst; rewrite H5 H8; try iExists (Ebinop op0 sla2.2 sla3.2 ty);
+        do 2 rewrite app_nil_l; iPureIntro; repeat split; auto; econstructor; eauto; rewrite <- H6;
+          auto; rewrite <- H9; rewrite comp_env_preserved; apply H3.
+    - iIntros "[_ HA]". iDestruct "HA" as (sla2)  "[HA [HB %]]". rewrite (surjective_pairing sla2).
+      iDestruct (H0 with "HA") as "[% [% %]]". inversion H2.
+      destruct dst; simpl in *; subst; rewrite H3; try iExists (Ecast sla2.2 ty); iPureIntro;
+        rewrite app_nil_l; repeat split; auto; econstructor; eauto; rewrite <- H4; auto.
+    - iIntros "[_ [HA %]]". inversion H.
+      destruct dst; simpl in *; subst; try iExists (Esizeof ty1 ty); iPureIntro; repeat split; eauto;
+        pose (P := comp_env_preserved); simpl in P; rewrite <- P; apply eval_Esizeof.
+    - iIntros "[_ [HA %]]". inversion H.
+      destruct dst; simpl in *; subst; try iExists (Ealignof ty1 ty); iPureIntro; repeat split; eauto;
+        pose (P := comp_env_preserved); simpl in P; rewrite <- P; constructor.
+    - iIntros "[_ %]". contradiction H.
+    - iIntros "[_ [_ %]]". inversion H0. iPureIntro. repeat split; auto. constructor. apply H.
+    - iIntros "[_ [_ %]]". inversion H1. iPureIntro. repeat split; auto.
+      apply eval_Evar_global; auto.
+      rewrite symbols_preserved; auto.
+    - iIntros "[_ HA]". iDestruct "HA" as (sla2)  "[HA [HB %]]". rewrite (surjective_pairing sla2).
+      iDestruct (H0 with "HA") as "[% [% %]]". inversion H1. iPureIntro. subst. repeat split.
+      rewrite app_nil_r. apply H2. rewrite typeof_Ederef'; auto. apply eval_Ederef'; auto. 
+    - iIntros "[_ HA]". iDestruct "HA" as (sla2)  "[HA [HB %]]". rewrite (surjective_pairing sla2).
+      iDestruct (H0 with "HA") as "[% [% %]]". inversion H4. subst. iPureIntro. repeat split.
+      rewrite app_nil_r. apply H5. rewrite <- comp_env_preserved in *. rewrite H6 in H1.
+      eapply eval_Efield_struct; eauto.
+    - iIntros "[_ HA]". iDestruct "HA" as (sla2)  "[HA [HB %]]". rewrite (surjective_pairing sla2).
+      iDestruct (H0 with "HA") as "[% [% %]]". inversion H3. subst. iPureIntro. repeat split.
+      rewrite app_nil_r. apply H4. rewrite <- comp_env_preserved in *. rewrite H5 in H1.
+      eapply eval_Efield_union; eauto.
 Qed.
    
 Lemma tr_simple_rvalue:
@@ -418,9 +420,9 @@ Lemma tr_simple_exprlist:
   ⌜ sl = nil /\ eval_exprlist tge e le m al tyl vl ⌝.
 Proof.
   induction rl.
-  - iIntros. inversion a.
+  - iIntros. destruct a. inversion H0.
     iPureIntro. repeat split; eauto. inversion a0. constructor.
-  - simpl. iIntros (? ?) "HA". iIntros (? ? ? ?) "%". iDestruct "HA" as (sla2 slal3) "[HA [HB %]]".
+  - simpl. iIntros (? ?) "[_ HA]". iIntros (? ? ? ?) "%". iDestruct "HA" as (sla2 slal3) "[HA [HB %]]".
     rewrite (surjective_pairing slal3).
     iDestruct (IHrl with "HB") as "HC".
     inversion a3. subst.
@@ -451,12 +453,13 @@ Lemma tr_expr_leftcontext_rec:
  (
   forall from to C, leftcontext from to C ->
   forall le e dst sl a,
-  tr_expr le dst (C e) (sl,a)-∗
+  tr_expr le dst (C e) (sl,a) -∗
   ∃ dst' sl1 sl2 a',
-  tr_expr le dst' e (sl1,a')  ∗ ⌜ sl = sl1 ++ sl2 ⌝
+  tr_expr le dst' e (sl1,a')
+  ∗ ⌜ sl = sl1 ++ sl2 ⌝
   ∗ (∀ le' e' sl3,
-        tr_expr le' dst' e' (sl3,a') -∗
-        (∀ id, (\s id -∗ False) -∗ ⌜ le'!id = le!id ⌝) -∗
+        (tr_expr le' dst' e' (sl3,a') ∧
+        (∀ id, (\s id -∗ False) -∗ ⌜ le'!id = le!id ⌝)) -∗
         \⌜ Csyntax.typeof e' = Csyntax.typeof e ⌝ -∗
         tr_expr le' dst (C e') ((sl3 ++ sl2),a))
  ) /\ (
@@ -467,8 +470,8 @@ Lemma tr_expr_leftcontext_rec:
   tr_expr le dst' e (sl1,a')
   ∗ ⌜sl = sl1 ++ sl2⌝
   ∗ (∀ le' e' sl3,
-        tr_expr le' dst' e' (sl3,a') -∗
-        (∀ id, (\s id -∗ False) -∗ ⌜ le'!id = le!id⌝) -∗
+        (tr_expr le' dst' e' (sl3,a') ∧
+        (∀ id, (\s id -∗ False) -∗ ⌜ le'!id = le!id⌝)) -∗
         \⌜ Csyntax.typeof e' = Csyntax.typeof e ⌝ -∗
         tr_exprlist le' (C e') ((sl3 ++ sl2),a))
 ).
@@ -483,8 +486,8 @@ Theorem tr_expr_leftcontext:
   tr_expr le dst' r (sl1,a')
   ∗ ⌜ sl = sl1 ++ sl2 ⌝
   ∗ (∀ le' r' sl3,
-        tr_expr le' dst' r' (sl3,a') -∗
-        (∀ id, (\s id -∗ False) -∗ ⌜ le'!id = le!id ⌝) -∗
+        (tr_expr le' dst' r' (sl3,a') ∧
+        (∀ id, (\s id -∗ False) -∗ ⌜ le'!id = le!id ⌝)) -∗
         \⌜ Csyntax.typeof r' = Csyntax.typeof r ⌝ -∗
         tr_expr le' dst (C r') ((sl3 ++ sl2),a)).
 Proof.
@@ -501,12 +504,33 @@ Theorem tr_top_leftcontext:
   tr_top tge e le m dst' r sl1 a'
   ∗ ⌜ sl = sl1 ++ sl2 ⌝
   ∗ (∀ le' m' r' sl3,
-        tr_expr le' dst' r' (sl3,a') -∗
-        (∀ id, (\s id -∗ False) -∗ ⌜le'!id = le!id ⌝) -∗
-        ⌜ Csyntax.typeof r' = Csyntax.typeof r ⌝ -∗
+        (tr_expr le' dst' r' (sl3,a') ∧
+        (∀ id, (\s id -∗ False) -∗ ⌜le'!id = le!id ⌝)) -∗
+        \⌜ Csyntax.typeof r' = Csyntax.typeof r ⌝ -∗
         tr_top tge e le' m' dst (C r') (sl3 ++ sl2) a).
 Proof.
-Admitted.
+  iIntros (? ? ? ? ? ? ?) "HA".
+  iDestruct "HA" as "[HA|%]". iIntros (r C H0 H1).
+  - subst. exploit tr_expr_leftcontext; eauto. intro.
+    iDestruct (H with "HA") as (dst' sl1 sl2 a') "[HA [% HC]]".
+    iExists dst', sl1, sl2, a'.
+    iSplitL "HA". iLeft.
+    + iApply "HA".
+    + iSplit; eauto. iIntros "* HA HB". iLeft. unfold tr_top_base.
+      iApply ("HC" with "[HA] [HB]"); eauto.
+  - iIntros (r C H0 H1). unfold tr_top_val_val in H.
+    destruct sl; auto. destruct H as (v&ty&P0&P1&P2&P3). subst.
+    inv H1; inv H0.
+    + iExists For_val, _, _, _. repeat iSplitL.
+      * iRight. iPureIntro. unfold tr_top_val_val. instantiate (3 := nil). simpl.
+        exists v, (typeof a). split; eauto.
+      * eauto.
+      * iIntros "* HA %".
+        rewrite <- app_nil_end. iLeft. unfold tr_top_base.
+        destruct r'; simpl; iDestruct "HA" as "[HA _]";
+          iDestruct "HA" as "[HC HA]"; iSplitL "HC"; eauto.
+    + inversion H.
+Qed.
 
 (** Semantics of smart constructors *)
 
@@ -635,6 +659,18 @@ Proof.
   eapply star_right. apply IHsl. constructor. traceEq.
 Qed.
 
+Lemma test3 (P Q : iProp) : (emp ⊢ P -∗ Q) -> (P ⊢ Q).
+Proof. intro.
+  iIntros "HA". iDestruct H as "HB". iApply "HB"; eauto.
+Qed.
+
+Lemma test4 : forall (P Q : iProp) tmps,
+    (P ∗ Q) () tmps -> exists (tmp0 tmp1 : heap),
+      P () tmp0 /\ Q () tmp1 /\ tmp0  ##ₘ tmp1 /\ tmps = tmp0 \u tmp1.
+Proof.
+  MonPred.unseal. intros. destruct H as (h0&h1&P0&P1&P2&P3). repeat eexists; eauto.
+Qed.
+
 Lemma step_tr_rvalof:
   forall ty m b ofs t v e le a sl a' f k,
   Csem.deref_loc ge ty m b ofs t v ->
@@ -648,40 +684,61 @@ Lemma step_tr_rvalof:
   /\ typeof a' = typeof a ⌝
   ∗ ∀ x, (\s x -∗ False) -∗ ⌜ le'!x = le!x ⌝.
 Proof.
-Admitted.
+  iIntros (? ? ? ? ? ? ? ? ? ? ? ? ? H0 H1) "HA %". unfold tr_rvalof.
+  destruct (type_is_volatile ty) eqn:?.
+  - iDestruct "HA" as  (t1) "[% HA]". inversion H. subst. clear H.
+    iExists (Maps.PTree.set t1 v le). iSplitR.
+    + iPureIntro. simpl. split. eapply star_two. econstructor. eapply step_make_set; eauto. traceEq.
+      split. constructor. apply Maps.PTree.gss.
+      reflexivity.
+    + iIntros (x) "HB". iStopProof. apply test3. apply test2. intros. apply Maps.PTree.gso.
+      intro. apply (soundness1 _ tmps). iIntros "HA". apply soundness3 in H.
+      iDestruct (H with "HA") as "[HA HB]". iDestruct ("HB" with "[HA]") as "HA".
+      iExists (typeof a). rewrite H2. iApply "HA". iApply "HA".
+  - iDestruct "HA" as "%". inversion H; subst. clear H.
+    exploit deref_loc_translated; eauto. intro.
+    unfold chunk_for_volatile_type in H. rewrite Heqb0 in H. destruct H. subst.
+    iExists le. iSplit; eauto.
+    iPureIntro. split.  apply star_refl.
+    split. eapply eval_Elvalue; eauto.
+    reflexivity.
+Qed.
+    
+    
 
+    
 (** Matching between continuations *)
 
 Inductive match_cont : Csem.cont -> cont -> Prop :=
   | match_Kstop:
       match_cont Csem.Kstop Kstop
-  | match_Kseq: forall s k ts tk tmp,
-      tr_stmt s ts () tmp ->
+  | match_Kseq: forall s k ts tk,
+      tr_stmt s ts ->
       match_cont k tk ->
       match_cont (Csem.Kseq s k) (Kseq ts tk)
-  | match_Kwhile2: forall r s k s' ts tk tmp tmp',
-      tr_if r Sskip Sbreak s' () tmp->
-      tr_stmt s ts () tmp' ->
+  | match_Kwhile2: forall r s k s' ts tk,
+      tr_if r Sskip Sbreak s' ->
+      tr_stmt s ts ->
       match_cont k tk ->
       match_cont (Csem.Kwhile2 r s k)
                  (Kloop1 (Ssequence s' ts) Sskip tk)
-  | match_Kdowhile1: forall r s k s' ts tk tmp,
-      tr_if r Sskip Sbreak s' () tmp ->
-      tr_stmt s ts () tmp ->
+  | match_Kdowhile1: forall r s k s' ts tk,
+      tr_if r Sskip Sbreak s' ->
+      tr_stmt s ts ->
       match_cont k tk ->
       match_cont (Csem.Kdowhile1 r s k)
                  (Kloop1 ts s' tk)
-  | match_Kfor3: forall r s3 s k ts3 s' ts tk tmp tmp' tmp'',
-      tr_if r Sskip Sbreak s' () tmp->
-      tr_stmt s3 ts3 () tmp' ->
-      tr_stmt s ts () tmp'' ->
+  | match_Kfor3: forall r s3 s k ts3 s' ts tk,
+      tr_if r Sskip Sbreak s' ->
+      tr_stmt s3 ts3 ->
+      tr_stmt s ts ->
       match_cont k tk ->
       match_cont (Csem.Kfor3 r s3 s k)
                  (Kloop1 (Ssequence s' ts) ts3 tk)
-  | match_Kfor4: forall r s3 s k ts3 s' ts tk tmp tmp' tmp'',
-      tr_if r Sskip Sbreak s' () tmp ->
-      tr_stmt s3 ts3 () tmp' ->
-      tr_stmt s ts () tmp'' ->
+  | match_Kfor4: forall r s3 s k ts3 s' ts tk,
+      tr_if r Sskip Sbreak s' ->
+      tr_stmt s3 ts3 ->
+      tr_stmt s ts ->
       match_cont k tk ->
       match_cont (Csem.Kfor4 r s3 s k)
                  (Kloop2 (Ssequence s' ts) ts3 tk)
@@ -712,36 +769,37 @@ with match_cont_exp : destination -> expr -> Csem.cont -> cont -> Prop :=
   | match_Kifthenelse_empty: forall a k tk,
       match_cont k tk ->
       match_cont_exp For_val a (Csem.Kifthenelse Csyntax.Sskip Csyntax.Sskip k) (Kseq Sskip tk)
-  | match_Kifthenelse_1: forall a s1 s2 k ts1 ts2 tk tmp tmp',
-      tr_stmt s1 ts1 () tmp -> tr_stmt s2 ts2 () tmp' ->
+  | match_Kifthenelse_1: forall a s1 s2 k ts1 ts2 tk,
+      tr_stmt s1 ts1 ->
+      tr_stmt s2 ts2 ->
       match_cont k tk ->
       match_cont_exp For_val a (Csem.Kifthenelse s1 s2 k) (Kseq (Sifthenelse a ts1 ts2) tk)
-  | match_Kwhile1: forall r s k s' a ts tk tmp tmp',
-      tr_if r Sskip Sbreak s' () tmp ->
-      tr_stmt s ts () tmp' ->
+  | match_Kwhile1: forall r s k s' a ts tk,
+      tr_if r Sskip Sbreak s' ->
+      tr_stmt s ts ->
       match_cont k tk ->
       match_cont_exp For_val a
          (Csem.Kwhile1 r s k)
          (Kseq (makeif a Sskip Sbreak)
            (Kseq ts (Kloop1 (Ssequence s' ts) Sskip tk)))
-  | match_Kdowhile2: forall r s k s' a ts tk tmp tmp',
-      tr_if r Sskip Sbreak s' () tmp ->
-      tr_stmt s ts () tmp' ->
+  | match_Kdowhile2: forall r s k s' a ts tk,
+      tr_if r Sskip Sbreak s' ->
+      tr_stmt s ts ->
       match_cont k tk ->
       match_cont_exp For_val a
         (Csem.Kdowhile2 r s k)
         (Kseq (makeif a Sskip Sbreak) (Kloop2 ts s' tk))
-  | match_Kfor2: forall r s3 s k s' a ts3 ts tk tmp tmp' tmp'',
-      tr_if r Sskip Sbreak s' () tmp ->
-      tr_stmt s3 ts3 () tmp' ->
-      tr_stmt s ts () tmp'' ->
+  | match_Kfor2: forall r s3 s k s' a ts3 ts tk,
+      tr_if r Sskip Sbreak s' ->
+      tr_stmt s3 ts3 ->
+      tr_stmt s ts ->
       match_cont k tk ->
       match_cont_exp For_val a
         (Csem.Kfor2 r s3 s k)
         (Kseq (makeif a Sskip Sbreak)
           (Kseq ts (Kloop1 (Ssequence s' ts) ts3 tk)))
-  | match_Kswitch1: forall ls k a tls tk tmp,
-      tr_lblstmts ls tls () tmp ->
+  | match_Kswitch1: forall ls k a tls tk,
+      tr_lblstmts ls tls ->
       match_cont k tk ->
       match_cont_exp For_val a (Csem.Kswitch1 ls k) (Kseq (Sswitch a tls) tk)
   | match_Kreturn: forall k a tk,
@@ -766,9 +824,9 @@ Inductive match_states: Csem.state -> Clight.state -> Prop :=
       match_cont_exp dest a k tk ->
       match_states (Csem.ExprState f r k e m)
                    (State tf Sskip (Kseqlist sl tk) e le m)
-  | match_regularstates: forall f s k e m tf ts tk le tmp,
+  | match_regularstates: forall f s k e m tf ts tk le,
       tr_function f tf ->
-      tr_stmt s ts () tmp ->
+      tr_stmt s ts ->
       match_cont k tk ->
       match_states (Csem.State f s k e m)
                    (State tf ts tk e le m)
@@ -788,17 +846,40 @@ Inductive match_states: Csem.state -> Clight.state -> Prop :=
 
 Lemma tr_select_switch:
   forall n ls tls,
-  tr_lblstmts ls tls -∗
+  tr_lblstmts ls tls ->
   tr_lblstmts (Csem.select_switch n ls) (select_switch n tls).
 Proof.
-Admitted.
+ assert (DFL: forall ls tls,
+      tr_lblstmts ls tls ->
+      tr_lblstmts (Csem.select_switch_default ls) (select_switch_default tls)).
+  { induction 1; simpl. constructor. destruct c; auto. constructor; auto. }
+  assert (CASE: forall n ls tls,
+      tr_lblstmts ls tls ->
+      match Csem.select_switch_case n ls with
+      | None =>
+          select_switch_case n tls = None
+      | Some ls' =>
+          exists tls', select_switch_case n tls = Some tls' /\ tr_lblstmts ls' tls'
+      end).
+  { induction 1; simpl; intros.
+    auto.
+    destruct c; auto. destruct (zeq z n); auto.
+    econstructor; split; eauto. constructor; auto. }
+  intros. unfold Csem.select_switch, select_switch.
+  specialize (CASE n ls tls H).
+  destruct (Csem.select_switch_case n ls) as [ls'|].
+  destruct CASE as [tls' [P Q]]. rewrite P. auto.
+  rewrite CASE. apply DFL; auto.
+Qed.
+
 
 Lemma tr_seq_of_labeled_statement:
   forall ls tls,
-  tr_lblstmts ls tls -∗
+  tr_lblstmts ls tls ->
   tr_stmt (Csem.seq_of_labeled_statement ls) (seq_of_labeled_statement tls).
 Proof.
-  Admitted.
+  induction 1; simpl; constructor; auto.
+Qed.
 
 (** Commutation between translation and the "find label" operation. *)
 
@@ -855,7 +936,12 @@ Qed.
 Lemma tr_rvalof_nolabel:
   forall ty a sl a', tr_rvalof ty a (sl,a') -∗ ⌜ nolabel_list sl ⌝.
 Proof.
-  Admitted.
+  iIntros (ty a sl a') "HA". unfold tr_rvalof. destruct (type_is_volatile ty) eqn:?.
+  - iDestruct "HA" as (t0) "[% HA]". inversion H; subst. clear H.
+    iStopProof. apply test3. apply test2. intros. simpl. split; auto.
+    apply make_set_nolabel.
+  - iDestruct "HA" as "%". inversion H; subst. iPureIntro. constructor.
+Qed.
 
 Lemma nolabel_do_set:
   forall sd a, nolabel_list (do_set sd a).
@@ -880,67 +966,550 @@ Ltac NoLabelTac :=
   | [ |- nolabel (makeif _ _ _) ] => apply makeif_nolabel; NoLabelTac
   | [ |- nolabel (make_set _ _) ] => apply make_set_nolabel
   | [ |- nolabel (make_assign _ _) ] => apply make_assign_nolabel
-  | [ |- nolabel _ ] => red; intros; simpl; auto
+  | [ |- nolabel_list (do_set _ _) ] => apply nolabel_do_set
+  | [ |- nolabel _ ] => iIntros; simpl; auto
   | [ |- _ /\ _ ] => split; NoLabelTac
   | _ => auto
   end.
 
-Lemma tr_find_label_expr:
-  (forall le dst r sl a, tr_expr le dst r (sl,a) -∗ ⌜ nolabel_list sl ⌝)
-/\(forall le rl sl al, tr_exprlist le rl (sl,al) -∗ ⌜ nolabel_list sl ⌝).
+Lemma test5 : forall (P Q : iProp) tmps, ((P ∧ Q) : iProp) () tmps -> (P () tmps ∧ Q () tmps).
 Proof.
-  Admitted.
-  
+  MonPred.unseal. intros. destruct H. split; auto. 
+Qed.
+
+Lemma tr_find_label_expr:
+  (forall r le dst sl a, tr_expr le dst r (sl,a) -∗ ⌜ nolabel_list sl ⌝)
+/\(forall rl le sl al, tr_exprlist le rl (sl,al) -∗ ⌜ nolabel_list sl ⌝).
+Proof.
+  apply tr_expr_exprlist; intros; iIntros "HA".
+  - destruct dst.
+    1-2 : iDestruct (tr_simple_expr_nil with "HA") as "HA";
+      iDestruct ("HA" with "[]") as "HA"; eauto;
+        iDestruct ("HA" with "[]") as "%"; eauto; rewrite H; auto.
+    iDestruct "HA" as "[_ HA]". iDestruct "HA" as (a0) "[_ [_ %]]".
+    simpl in *. rewrite H. iPureIntro. apply nolabel_do_set.
+  - destruct dst.
+    1-2 : iDestruct (tr_simple_expr_nil with "HA") as "HA";
+      iDestruct ("HA" with "[]") as "HA"; eauto;
+        iDestruct ("HA" with "[]") as "%"; eauto; rewrite H; auto.
+    iDestruct "HA" as "[_ [HA %]]".
+    simpl in *. inversion H; subst. iPureIntro. apply nolabel_do_set.
+  - destruct dst.
+    + iDestruct "HA" as "[_ HA]"; fold tr_expr. 
+      iDestruct "HA" as (sla2) "[HB [HA %]]". rewrite (surjective_pairing sla2).
+      iDestruct (H with "HB") as "%". inversion H0; subst. clear H0.
+      iPureIntro. NoLabelTac.
+    + iDestruct "HA" as "[_ HA]"; fold tr_expr. 
+      iDestruct "HA" as (sla2) "[HB [HA %]]". rewrite (surjective_pairing sla2).
+      iDestruct (H with "HB") as "%". inversion H0; subst. clear H0.
+      iPureIntro. NoLabelTac.
+    + iDestruct "HA" as "[_ HA]"; fold tr_expr. 
+      iDestruct "HA" as (sla2) "[HB [HA %]]". rewrite (surjective_pairing sla2).
+      iDestruct (H with "HB") as "%". inversion H0; subst. clear H0.
+      iPureIntro. NoLabelTac. 
+  - destruct dst.
+    + iDestruct "HA" as "[_ HA]"; fold tr_expr. 
+      iDestruct "HA" as (sla2 sl3) "[HB [HA [_ %]]]". rewrite (surjective_pairing sla2).
+      iDestruct (H with "HB") as "%". simpl in *. rewrite H0.
+      iDestruct (tr_rvalof_nolabel with "HA") as "%".
+      iPureIntro. NoLabelTac.
+    + iDestruct "HA" as "[_ HA]"; fold tr_expr. 
+      iDestruct "HA" as (sla2 sl3) "[HB [HA [_ %]]]". rewrite (surjective_pairing sla2).
+      iDestruct (H with "HB") as "%". simpl in *. rewrite H0.
+      iDestruct (tr_rvalof_nolabel with "HA") as "%".
+      iPureIntro. NoLabelTac.
+    + iDestruct "HA" as "[_ HA]"; fold tr_expr. 
+      iDestruct "HA" as (sla2 sl3) "[HB [HA [_ %]]]". rewrite (surjective_pairing sla2).
+      iDestruct (H with "HB") as "%". simpl in *. rewrite H0.
+      iDestruct (tr_rvalof_nolabel with "HA") as "%".
+      iPureIntro. NoLabelTac.
+  - destruct dst.
+    + iDestruct "HA" as "[_ HA]"; fold tr_expr. 
+      iDestruct "HA" as (sla2) "[HB [HA %]]". rewrite (surjective_pairing sla2).
+      inversion H0; subst.
+      iDestruct (H with "HB") as "%". simpl in *. 
+      iPureIntro. NoLabelTac.
+    + iDestruct "HA" as "[_ HA]"; fold tr_expr. 
+      iDestruct "HA" as (sla2) "[HB [HA %]]". rewrite (surjective_pairing sla2).
+      inversion H0; subst.
+      iDestruct (H with "HB") as "%". simpl in *. 
+      iPureIntro. NoLabelTac.
+    + iDestruct "HA" as "[_ HA]"; fold tr_expr. 
+      iDestruct "HA" as (sla2) "[HB [HA %]]". rewrite (surjective_pairing sla2).
+      inversion H0; subst.
+      iDestruct (H with "HB") as "%". simpl in *. 
+      iPureIntro. NoLabelTac.
+  - destruct dst.
+    + iDestruct "HA" as "[_ HA]"; fold tr_expr. 
+      iDestruct "HA" as (sla2) "[HB [HA %]]". rewrite (surjective_pairing sla2).
+      inversion H0; subst.
+      iDestruct (H with "HB") as "%". simpl in *. 
+      iPureIntro. NoLabelTac.
+    + iDestruct "HA" as "[_ HA]"; fold tr_expr. 
+      iDestruct "HA" as (sla2) "[HB [HA %]]". rewrite (surjective_pairing sla2).
+      inversion H0; subst.
+      iDestruct (H with "HB") as "%". simpl in *. 
+      iPureIntro. NoLabelTac.
+    + iDestruct "HA" as "[_ HA]"; fold tr_expr. 
+      iDestruct "HA" as (sla2) "[HB [HA %]]". rewrite (surjective_pairing sla2).
+      inversion H0; subst.
+      iDestruct (H with "HB") as "%". simpl in *. 
+      iPureIntro. NoLabelTac.
+  - destruct dst.
+    + iDestruct "HA" as "[_ HA]"; fold tr_expr. 
+      iDestruct "HA" as (sla2) "[HB [HA %]]". rewrite (surjective_pairing sla2).
+      inversion H0; subst.
+      iDestruct (H with "HB") as "%". simpl in *. 
+      iPureIntro. NoLabelTac.
+    + iDestruct "HA" as "[_ HA]"; fold tr_expr. 
+      iDestruct "HA" as (sla2) "[HB [HA %]]". rewrite (surjective_pairing sla2).
+      inversion H0; subst.
+      iDestruct (H with "HB") as "%". simpl in *. 
+      iPureIntro. NoLabelTac.
+    + iDestruct "HA" as "[_ HA]"; fold tr_expr. 
+      iDestruct "HA" as (sla2) "[HB [HA %]]". rewrite (surjective_pairing sla2).
+      inversion H0; subst.
+      iDestruct (H with "HB") as "%". simpl in *. 
+      iPureIntro. NoLabelTac.
+  - destruct dst.
+    + iDestruct "HA" as "[_ HA]"; fold tr_expr. 
+      iDestruct "HA" as (sla2 sla3) "[HB [HA [_ %]]]". rewrite (surjective_pairing sla2).
+      rewrite (surjective_pairing sla3).
+      inversion H1; subst.
+      iDestruct (H with "HB") as "%".
+      iDestruct (H0 with "HA") as "%". 
+      iPureIntro. NoLabelTac.
+    + iDestruct "HA" as "[_ HA]"; fold tr_expr. 
+      iDestruct "HA" as (sla2 sla3) "[HB [HA [_ %]]]". rewrite (surjective_pairing sla2).
+      rewrite (surjective_pairing sla3).
+      inversion H1; subst.
+      iDestruct (H with "HB") as "%".
+      iDestruct (H0 with "HA") as "%". 
+      iPureIntro. NoLabelTac.
+    + iDestruct "HA" as "[_ HA]"; fold tr_expr. 
+      iDestruct "HA" as (sla2 sla3) "[HB [HA [_ %]]]". rewrite (surjective_pairing sla2).
+      rewrite (surjective_pairing sla3).
+      inversion H1; subst.
+      iDestruct (H with "HB") as "%".
+      iDestruct (H0 with "HA") as "%". 
+      iPureIntro. NoLabelTac.
+  - destruct dst.
+    + iDestruct "HA" as "[_ HA]"; fold tr_expr. 
+      iDestruct "HA" as (sla2) "[HB [HA %]]". rewrite (surjective_pairing sla2).
+      inversion H0; subst.
+      iDestruct (H with "HB") as "%". simpl in *. 
+      iPureIntro. NoLabelTac.
+    + iDestruct "HA" as "[_ HA]"; fold tr_expr. 
+      iDestruct "HA" as (sla2) "[HB [HA %]]". rewrite (surjective_pairing sla2).
+      inversion H0; subst.
+      iDestruct (H with "HB") as "%". simpl in *. 
+      iPureIntro. NoLabelTac.
+    + iDestruct "HA" as "[_ HA]"; fold tr_expr. 
+      iDestruct "HA" as (sla2) "[HB [HA %]]". rewrite (surjective_pairing sla2).
+      inversion H0; subst.
+      iDestruct (H with "HB") as "%". simpl in *. 
+      iPureIntro. NoLabelTac.
+  - destruct dst.
+    + iDestruct "HA" as "[_ HA]"; fold tr_expr. 
+      iDestruct "HA" as (sla2 sla3 t0) "[HB [HA [HC %]]]". rewrite (surjective_pairing sla2).
+      rewrite (surjective_pairing sla3). iDestruct ("HA" with "HC") as "HA".
+      inversion H1; subst.
+      iDestruct (H with "HB") as "%".
+      iDestruct (H0 with "HA") as "%". 
+      iPureIntro. NoLabelTac. red. unfold find_label. auto.
+    + iDestruct "HA" as "[_ HA]"; fold tr_expr. 
+      iDestruct "HA" as (sla2 sla3) "[HB [HA %]]". rewrite (surjective_pairing sla2).
+      rewrite (surjective_pairing sla3). 
+      simpl in *; subst.
+      iDestruct (H with "HB") as "%".
+      iDestruct (H0 with "HA") as "%". 
+      iPureIntro. NoLabelTac. red. unfold find_label. auto.
+    + iDestruct "HA" as "[_ HA]"; fold tr_expr. 
+      iDestruct "HA" as (sla2 sla3) "[HB [HA [HC %]]]". rewrite (surjective_pairing sla2).
+      rewrite (surjective_pairing sla3). iDestruct ("HA" with "HC") as "HA".
+      simpl in *; subst.
+      iDestruct (H with "HB") as "%".
+      iDestruct (H0 with "HA") as "%". 
+      iPureIntro. NoLabelTac.
+  - destruct dst.
+    + iDestruct "HA" as "[_ HA]"; fold tr_expr. 
+      iDestruct "HA" as (sla2 sla3 t0) "[HB [HA [HC %]]]". rewrite (surjective_pairing sla2).
+      rewrite (surjective_pairing sla3). iDestruct ("HA" with "HC") as "HA".
+      inversion H1; subst.
+      iDestruct (H with "HB") as "%".
+      iDestruct (H0 with "HA") as "%". 
+      iPureIntro. NoLabelTac. red. unfold find_label. auto.
+    + iDestruct "HA" as "[_ HA]"; fold tr_expr. 
+      iDestruct "HA" as (sla2 sla3) "[HB [HA %]]". rewrite (surjective_pairing sla2).
+      rewrite (surjective_pairing sla3). 
+      simpl in *; subst.
+      iDestruct (H with "HB") as "%".
+      iDestruct (H0 with "HA") as "%". 
+      iPureIntro. NoLabelTac. red. unfold find_label. auto.
+    + iDestruct "HA" as "[_ HA]"; fold tr_expr. 
+      iDestruct "HA" as (sla2 sla3) "[HB [HA [HC %]]]". rewrite (surjective_pairing sla2).
+      rewrite (surjective_pairing sla3). iDestruct ("HA" with "HC") as "HA".
+      simpl in *; subst.
+      iDestruct (H with "HB") as "%".
+      iDestruct (H0 with "HA") as "%". 
+      iPureIntro. NoLabelTac.
+  - destruct dst.
+    + iDestruct "HA" as "[_ HA]"; fold tr_expr.
+      iDestruct "HA" as (sla2 sla3 sla4 t0) "[HA [HB [HC %]]]".
+      inversion H2; subst. clear H2. rewrite (surjective_pairing sla2).
+      iDestruct (H with "HA") as "%". iClear "HA".
+      iDestruct ("HC" with "HB") as "HA".
+      iStopProof. apply test3. apply test2. intros. apply test5 in H3 as (P0&P1).
+      apply (soundness1 _ tmps). apply soundness3 in P0. iIntros "HA".
+      iDestruct (P0 with "HA") as "HA".
+      rewrite (surjective_pairing sla3). iDestruct (H0 with "HA") as "%".
+      iPureIntro.
+      apply (soundness1 _ tmps). apply soundness3 in P1. iIntros "HA".
+      iDestruct (P1 with "HA") as "HA".
+      rewrite (surjective_pairing sla4). iDestruct (H1 with "HA") as "%".
+      simpl in *; subst. iPureIntro. NoLabelTac.
+    + iDestruct "HA" as "[_ HA]"; fold tr_expr.
+      iDestruct "HA" as (sla2 sla3 sla4) "[HA [HB [HC %]]]".
+      simpl in *; subst. rewrite (surjective_pairing sla2). rewrite (surjective_pairing sla3).
+      rewrite (surjective_pairing sla4).
+      iDestruct (H with "HA") as "%". iClear "HA".
+      iDestruct (H0 with "HB") as "%". iClear "HB".
+      iDestruct (H1 with "HC") as "%". iClear "HC".
+      simpl in *; subst. iPureIntro. NoLabelTac.
+    + iDestruct "HA" as "[_ HA]"; fold tr_expr.
+      iDestruct "HA" as (sla2 sla3 sla4 t0) "[HA [HB [HC %]]]".
+      inversion H2; subst. clear H2. rewrite (surjective_pairing sla2).
+      iDestruct (H with "HA") as "%". iClear "HA".
+      iDestruct ("HC" with "HB") as "HA".
+      iStopProof. apply test3. apply test2. intros. apply test5 in H4 as (P0&P1).
+      apply (soundness1 _ tmps). apply soundness3 in P0. iIntros "HA".
+      iDestruct (P0 with "HA") as "HA".
+      rewrite (surjective_pairing sla3). iDestruct (H0 with "HA") as "%".
+      iPureIntro.
+      apply (soundness1 _ tmps). apply soundness3 in P1. iIntros "HA".
+      iDestruct (P1 with "HA") as "HA".
+      rewrite (surjective_pairing sla4). iDestruct (H1 with "HA") as "%".
+      simpl in *; subst. iPureIntro. NoLabelTac.      
+  - destruct dst.
+    1-2 : iDestruct (tr_simple_expr_nil with "HA") as "HA";
+      iDestruct ("HA" with "[]") as "HA"; eauto;
+        iDestruct ("HA" with "[]") as "%"; eauto; rewrite H; auto.
+    iDestruct "HA" as "[_ HA]". iDestruct "HA" as "[_ %]".
+    simpl in *. inversion H; subst. iPureIntro. apply nolabel_do_set.      
+  - destruct dst.
+    1-2 : iDestruct (tr_simple_expr_nil with "HA") as "HA";
+      iDestruct ("HA" with "[]") as "HA"; eauto;
+        iDestruct ("HA" with "[]") as "%"; eauto; rewrite H; auto.
+    iDestruct "HA" as "[_ HA]". iDestruct "HA" as "[_ %]".
+    simpl in *. inversion H; subst. iPureIntro. apply nolabel_do_set.
+  - destruct dst.
+    + iDestruct "HA" as "[_ HA]"; fold tr_expr. 
+      iDestruct "HA" as (sla2 sla3) "[HB [HA HC]]". rewrite (surjective_pairing sla2).
+      rewrite (surjective_pairing sla3). 
+      iDestruct (H with "HB") as "%".
+      iDestruct (H0 with "HA") as "%".
+      iDestruct "HC" as "[[% %]|HC]".
+      * inversion H4.
+      * iDestruct "HC" as (t0) "[HC %]". simpl in *. subst. iPureIntro. NoLabelTac.
+        red. intros.  unfold find_label. reflexivity.
+    + iDestruct "HA" as "[_ HA]"; fold tr_expr. 
+      iDestruct "HA" as (sla2 sla3) "[HB [HA HC]]". rewrite (surjective_pairing sla2).
+      rewrite (surjective_pairing sla3). 
+      iDestruct (H with "HB") as "%".
+      iDestruct (H0 with "HA") as "%".
+      iDestruct "HC" as "[[% %]|HC]".
+      * simpl in *. subst. iPureIntro. NoLabelTac.
+      * iDestruct "HC" as (t0) "[HC %]". simpl in *. subst. iPureIntro. NoLabelTac.
+        red. intros.  unfold find_label. reflexivity.
+    + iDestruct "HA" as "[_ HA]"; fold tr_expr. 
+      iDestruct "HA" as (sla2 sla3) "[HB [HA HC]]". rewrite (surjective_pairing sla2).
+      rewrite (surjective_pairing sla3). 
+      iDestruct (H with "HB") as "%".
+      iDestruct (H0 with "HA") as "%".
+      iDestruct "HC" as "[[% %]|HC]".
+      * inversion H4.
+      * iDestruct "HC" as (t0) "[HC %]". simpl in *. subst. iPureIntro. NoLabelTac.
+        red. intros.  unfold find_label. reflexivity.
+  - destruct dst.
+    + iDestruct "HA" as "[_ HA]"; fold tr_expr. 
+      iDestruct "HA" as (sla2 sla3 sla4) "[HB [HA [HC HD]]]". rewrite (surjective_pairing sla2).
+      rewrite (surjective_pairing sla3). rewrite (surjective_pairing sla4). 
+      iDestruct (H with "HB") as "%".
+      iDestruct (H0 with "HA") as "%".
+      simpl. iDestruct (tr_rvalof_nolabel with "HC") as "%".
+      iDestruct "HD" as "[[% %]|HD]".
+      * inversion H4.
+      * iDestruct "HD" as (t0) "[HD %]". inversion H4. subst. iPureIntro. NoLabelTac.
+        red. intros. unfold find_label. reflexivity.
+    + iDestruct "HA" as "[_ HA]"; fold tr_expr. 
+      iDestruct "HA" as (sla2 sla3 sla4) "[HB [HA [HC HD]]]". rewrite (surjective_pairing sla2).
+      rewrite (surjective_pairing sla3). rewrite (surjective_pairing sla4). 
+      iDestruct (H with "HB") as "%".
+      iDestruct (H0 with "HA") as "%".
+      simpl. iDestruct (tr_rvalof_nolabel with "HC") as "%".
+      iDestruct "HD" as "[[% %]|HD]".
+      * rewrite H5. iPureIntro. NoLabelTac.
+      * iDestruct "HD" as (t0) "[HD %]". inversion H4. subst. iPureIntro. NoLabelTac.
+        red. intros. unfold find_label. reflexivity.
+    + iDestruct "HA" as "[_ HA]"; fold tr_expr. 
+      iDestruct "HA" as (sla2 sla3 sla4) "[HB [HA [HC HD]]]". rewrite (surjective_pairing sla2).
+      rewrite (surjective_pairing sla3). rewrite (surjective_pairing sla4). 
+      iDestruct (H with "HB") as "%".
+      iDestruct (H0 with "HA") as "%".
+      simpl. iDestruct (tr_rvalof_nolabel with "HC") as "%".
+      iDestruct "HD" as "[[% %]|HD]".
+      * inversion H4.
+      * iDestruct "HD" as (t0) "[HD %]". inversion H4. subst. iPureIntro. NoLabelTac.
+        red. intros. unfold find_label. reflexivity.
+  - destruct dst.
+    + iDestruct "HA" as "[_ [HA|HA]]"; fold tr_expr.
+      * iDestruct "HA" as (sla2 sla3) "[HB [HA %]]". rewrite (surjective_pairing sla2).
+        rewrite (surjective_pairing sla3). simpl. iDestruct (tr_rvalof_nolabel with "HA") as "%".
+        iDestruct (H with "HB") as "%". simpl in *; subst. iPureIntro. NoLabelTac.
+      * iDestruct "HA" as (sla2 t0) "[HB [HA %]]". rewrite (surjective_pairing sla2).
+        inversion H0; subst.
+        iDestruct (H with "HB") as "%". simpl in *; subst. iPureIntro. NoLabelTac.
+    + iDestruct "HA" as "[_ [HA|HA]]"; fold tr_expr.
+      * iDestruct "HA" as (sla2 sla3) "[HB [HA %]]". rewrite (surjective_pairing sla2).
+        rewrite (surjective_pairing sla3). simpl. iDestruct (tr_rvalof_nolabel with "HA") as "%".
+        iDestruct (H with "HB") as "%". simpl in *; subst. iPureIntro. NoLabelTac.
+      * iDestruct "HA" as (sla2 t0) "[HB [HA %]]". rewrite (surjective_pairing sla2).
+        inversion H0; subst.
+        iDestruct (H with "HB") as "%". simpl in *; subst. iPureIntro. NoLabelTac.
+    + iDestruct "HA" as "[_ [HA|HA]]"; fold tr_expr.
+      * iDestruct "HA" as (sla2 sla3) "[HB [HA %]]". rewrite (surjective_pairing sla2).
+        rewrite (surjective_pairing sla3). simpl. iDestruct (tr_rvalof_nolabel with "HA") as "%".
+        iDestruct (H with "HB") as "%". simpl in *; subst. iPureIntro. NoLabelTac.
+      * iDestruct "HA" as (sla2 t0) "[HB [HA %]]". rewrite (surjective_pairing sla2).
+        inversion H0; subst.
+        iDestruct (H with "HB") as "%". simpl in *; subst. iPureIntro. NoLabelTac.
+  - destruct dst.
+    + iDestruct "HA" as "[_ HA]"; fold tr_expr.
+      iDestruct "HA" as (sla2 sl3) "[HB [HA [_ %]]]". rewrite (surjective_pairing sla2).
+      simpl. iDestruct (H with "HB") as "%". simpl in *; subst.
+      iDestruct (H0 with "[HA]") as "%".
+      * iApply "HA". trivial.
+      * iPureIntro. NoLabelTac.
+    + iDestruct "HA" as "[_ HA]"; fold tr_expr.
+      iDestruct "HA" as (sla2 sl3) "[HB [HA [_ %]]]". rewrite (surjective_pairing sla2).
+      simpl. iDestruct (H with "HB") as "%". simpl in *; subst.
+      iDestruct (H0 with "[HA]") as "%".
+      * iApply "HA". trivial.
+      * iPureIntro. NoLabelTac.
+    + iDestruct "HA" as "[_ HA]"; fold tr_expr.
+      iDestruct "HA" as (sla2 sl3) "[HB [HA [HC %]]]". rewrite (surjective_pairing sla2).
+      simpl. iDestruct (H with "HB") as "%". simpl in *; subst.
+      iDestruct (H0 with "[HA HC]") as "%".
+      * iApply "HA". trivial.
+      * iPureIntro. NoLabelTac.
+  - destruct dst.
+    + iDestruct "HA" as "[_ HA]"; fold tr_expr; fold tr_exprlist.
+      iDestruct "HA" as (sla2 slal3 t0) "[HB [HA [HC [_ %]]]]". rewrite (surjective_pairing sla2).
+      rewrite (surjective_pairing slal3). inversion H1; subst.
+      iDestruct (H with "HB") as "%".
+      iDestruct (H0 with "HA") as "%".
+      iPureIntro. NoLabelTac.
+      red. intros. unfold find_label. reflexivity.
+    + iDestruct "HA" as "[_ HA]"; fold tr_expr; fold tr_exprlist.
+      iDestruct "HA" as (sla2 slal3) "[HB [HA %]]". rewrite (surjective_pairing sla2).
+      rewrite (surjective_pairing slal3). simpl in *; subst.
+      iDestruct (H with "HB") as "%".
+      iDestruct (H0 with "HA") as "%".
+      iPureIntro. NoLabelTac.
+      red. intros. unfold find_label. reflexivity.
+    + iDestruct "HA" as "[_ HA]"; fold tr_expr; fold tr_exprlist.
+      iDestruct "HA" as (sla2 slal3 t0) "[HB [HA [HC [_ %]]]]". rewrite (surjective_pairing sla2).
+      rewrite (surjective_pairing slal3). inversion H1; subst.
+      iDestruct (H with "HB") as "%".
+      iDestruct (H0 with "HA") as "%".
+      iPureIntro. NoLabelTac.
+      red. intros. unfold find_label. reflexivity.
+  - destruct dst.
+    + iDestruct "HA" as "[_ HA]"; fold tr_expr; fold tr_exprlist.
+      iDestruct "HA" as (slal2 t0) "[HB [HA [_ %]]]". rewrite (surjective_pairing slal2).
+      inversion H0; subst. iDestruct (H with "HB") as "%".
+      iPureIntro. NoLabelTac.
+      red. intros. unfold find_label. reflexivity.
+    + iDestruct "HA" as "[_ HA]"; fold tr_expr; fold tr_exprlist.
+      iDestruct "HA" as (slal2) "[HB %]". rewrite (surjective_pairing slal2).
+      simpl in *; subst. iDestruct (H with "HB") as "%".
+      iPureIntro. NoLabelTac.
+      red. intros. unfold find_label. reflexivity.
+    + iDestruct "HA" as "[_ HA]"; fold tr_expr; fold tr_exprlist.
+      iDestruct "HA" as (slal2 t0) "[HB [HA [_ %]]]". rewrite (surjective_pairing slal2).
+      inversion H0; subst. iDestruct (H with "HB") as "%".
+      iPureIntro. NoLabelTac.
+      red. intros. unfold find_label. reflexivity.
+  - destruct dst; iDestruct "HA" as "[_ HA]"; iExFalso; iApply "HA".
+  - destruct dst.
+    + iDestruct "HA" as "[_ HA]"; fold tr_expr; fold tr_exprlist.
+      iDestruct "HA" as (a2 t0) "[HB [HA %]]". iDestruct ("HB" with "HA") as "HA". simpl.
+      iDestruct (H with "HA") as "%". iPureIntro. apply H1.
+    + iDestruct "HA" as "[_ HA]"; fold tr_expr; fold tr_exprlist.
+      iDestruct "HA" as (a2) "HA". simpl.
+      iDestruct (H with "HA") as "%". iPureIntro. apply H0.
+    + iDestruct "HA" as "[_ HA]"; fold tr_expr; fold tr_exprlist.
+      iDestruct "HA" as (a2 t0) "[HB HA]". iDestruct ("HB" with "HA") as "HA". simpl.
+      iDestruct (H with "HA") as "%". iPureIntro. apply H0.
+  - iDestruct "HA" as "[_ %]". inversion H. iPureIntro. NoLabelTac.
+  - iDestruct "HA" as "[_ HA]"; fold tr_expr; fold tr_exprlist.
+    iDestruct "HA" as (sla2 slal3) "[HA [HB %]]". inversion H1; subst.
+    rewrite (surjective_pairing sla2). rewrite (surjective_pairing slal3).
+    simpl. iDestruct (H with "HA") as "%". iDestruct (H0 with "HB") as "%".
+    iPureIntro. NoLabelTac.
+Qed.
+                                        
 Lemma tr_find_label_top:
   forall e le m dst r sl a,
     tr_top tge e le m dst r sl a -∗ ⌜ nolabel_list sl ⌝.
 Proof.
-  Admitted.
+  intros. iIntros "HA". unfold tr_top. iDestruct ("HA" with "") as "[HA|%]".
+  - unfold tr_top_base. epose tr_find_label_expr. destruct a0. iApply (H with "HA").
+  - unfold tr_top_val_val in H. destruct sl; auto.
+Qed.
 
 Lemma tr_find_label_expression:
-  forall r s a, tr_expression r s a -∗ ⌜ forall k, find_label lbl s k = None ⌝.
+  forall r s a, tr_expression r s a -> forall k, find_label lbl s k = None.
 Proof.
-Admitted.
+  intros. inv H.
+  assert (nolabel (makeseq sl)). apply makeseq_nolabel.
+  pose (H0 tge empty_env (Maps.PTree.empty val) Mem.empty).
+  apply soundness3 in m.
+  apply (soundness1 _ tmps). iIntros "HA". iDestruct (m with "HA") as "HA".
+  iApply tr_find_label_top; eauto.
+  apply H.
+Qed.
 
 Lemma tr_find_label_expr_stmt:
-  forall r s, tr_expr_stmt r s -∗ ⌜ forall k, find_label lbl s k = None ⌝.
+  forall r s, tr_expr_stmt r s -> forall k, find_label lbl s k = None.
 Proof.
-  Admitted.
+  intros. inv H.
+  assert (nolabel (makeseq sl)). apply makeseq_nolabel.
+  pose (H0 tge empty_env (Maps.PTree.empty val) Mem.empty).
+  apply soundness3 in m.
+  apply (soundness1 _ tmps). iIntros "HA". iDestruct (m with "HA") as "HA".
+  iApply tr_find_label_top; eauto.
+  apply H.
+Qed.
 
 Lemma tr_find_label_if:
-  forall r s, tr_if r Sskip Sbreak s -∗ ⌜ forall k, find_label lbl s k = None ⌝.
+  forall r s, tr_if r Sskip Sbreak s -> forall k, find_label lbl s k = None.
 Proof.
-Admitted.
-
-
+  intros. inv H.
+  assert (nolabel (makeseq (sl ++ makeif a Sskip Sbreak :: nil))).
+  apply makeseq_nolabel.
+  apply nolabel_list_app.
+  pose (H0 tge empty_env (Maps.PTree.empty val) Mem.empty).
+  apply soundness3 in m.
+  apply (soundness1 _ tmps). iIntros "HA". iDestruct (m with "HA") as "HA".
+  iApply tr_find_label_top; eauto.
+  simpl; split; auto. apply makeif_nolabel. red; simpl; auto. red; simpl; auto.
+  apply H.
+Qed.
 Lemma tr_find_label:
-  forall s k ts tk,
-    tr_stmt s ts -∗
-    ⌜ match_cont k tk ⌝ -∗
+  forall s k ts tk
+    (TR: tr_stmt s ts)
+    (MC: match_cont k tk),
   match Csem.find_label lbl s k with
   | None =>
-      ⌜ find_label lbl ts tk = None ⌝
+      find_label lbl ts tk = None
   | Some (s', k') =>
-      ∃ ts', ∃ tk',
-          ⌜ find_label lbl ts tk = Some (ts', tk') ⌝
-       ∗ tr_stmt s' ts'
-       ∗ ⌜match_cont k' tk'⌝
+      exists ts', exists tk',
+          find_label lbl ts tk = Some (ts', tk')
+       /\ tr_stmt s' ts'
+       /\ match_cont k' tk'
   end
 with tr_find_label_ls:
-  forall s k ts tk,
-    tr_lblstmts s ts -∗
-                ⌜ match_cont k tk ⌝-∗
+  forall s k ts tk
+    (TR: tr_lblstmts s ts)
+    (MC: match_cont k tk),
   match Csem.find_label_ls lbl s k with
   | None =>
-      ⌜ find_label_ls lbl ts tk = None ⌝
+      find_label_ls lbl ts tk = None
   | Some (s', k') =>
-      ∃ ts' tk',
-          ⌜ find_label_ls lbl ts tk = Some (ts', tk') ⌝
-       ∗ tr_stmt s' ts'
-       ∗ ⌜match_cont k' tk'⌝
+      exists ts', exists tk',
+          find_label_ls lbl ts tk = Some (ts', tk')
+       /\ tr_stmt s' ts'
+       /\ match_cont k' tk'
   end.
 Proof.
-Admitted.
+  induction s; intros; inversion TR; subst; clear TR; simpl.
+  auto.
+  eapply tr_find_label_expr_stmt; eauto.
+(* seq *)
+  exploit (IHs1 (Csem.Kseq s2 k)); eauto. constructor; eauto.
+  destruct (Csem.find_label lbl s1 (Csem.Kseq s2 k)) as [[s' k'] | ].
+  intros [ts' [tk' [A [B C]]]]. rewrite A. exists ts'; exists tk'; auto.
+  intro EQ. rewrite EQ. eapply IHs2; eauto.
+(* if empty *)
+  rename s' into sr.
+  rewrite (tr_find_label_expression _ _ _ H3).
+  auto.
+(* if not empty *)
+  rename s' into sr.
+  rewrite (tr_find_label_expression _ _ _ H2).
+  exploit (IHs1 k); eauto.
+  destruct (Csem.find_label lbl s1 k) as [[s' k'] | ].
+  intros [ts' [tk' [A [B C]]]]. rewrite A. exists ts'; exists tk'; intuition.
+  intro EQ. rewrite EQ. eapply IHs2; eauto.
+(* while *)
+  rename s' into sr.
+  rewrite (tr_find_label_if _ _ H1); auto.
+  exploit (IHs (Kwhile2 e s k)); eauto. econstructor; eauto.
+  destruct (Csem.find_label lbl s (Kwhile2 e s k)) as [[s' k'] | ].
+  intros [ts' [tk' [A [B C]]]]. rewrite A. exists ts'; exists tk'; intuition.
+  intro EQ. rewrite EQ. auto.
+(* dowhile *)
+  rename s' into sr.
+  rewrite (tr_find_label_if _ _ H1); auto.
+  exploit (IHs (Kdowhile1 e s k)); eauto. econstructor; eauto.
+  destruct (Csem.find_label lbl s (Kdowhile1 e s k)) as [[s' k'] | ].
+  intros [ts' [tk' [A [B C]]]]. rewrite A. exists ts'; exists tk'; intuition.
+  intro EQ. rewrite EQ. auto.
+(* for skip *)
+  rename s' into sr.
+  rewrite (tr_find_label_if _ _ H4); auto.
+  exploit (IHs3 (Csem.Kfor3 e s2 s3 k)); eauto. econstructor; eauto.
+  destruct (Csem.find_label lbl s3 (Csem.Kfor3 e s2 s3 k)) as [[s' k'] | ].
+  intros [ts' [tk' [A [B C]]]]. rewrite A. exists ts'; exists tk'; intuition.
+  intro EQ. rewrite EQ.
+  exploit (IHs2 (Csem.Kfor4 e s2 s3 k)); eauto. econstructor; eauto.
+(* for not skip *)
+  rename s' into sr.
+  rewrite (tr_find_label_if _ _ H3); auto.
+  exploit (IHs1 (Csem.Kseq (Csyntax.Sfor Csyntax.Sskip e s2 s3) k)); eauto.
+    econstructor; eauto. econstructor; eauto.
+  destruct (Csem.find_label lbl s1
+               (Csem.Kseq (Csyntax.Sfor Csyntax.Sskip e s2 s3) k)) as [[s' k'] | ].
+  intros [ts' [tk' [A [B C]]]]. rewrite A. exists ts'; exists tk'; intuition.
+  intro EQ; rewrite EQ.
+  exploit (IHs3 (Csem.Kfor3 e s2 s3 k)); eauto. econstructor; eauto.
+  destruct (Csem.find_label lbl s3 (Csem.Kfor3 e s2 s3 k)) as [[s'' k''] | ].
+  intros [ts' [tk' [A [B C]]]]. rewrite A. exists ts'; exists tk'; intuition.
+  intro EQ'. rewrite EQ'.
+  exploit (IHs2 (Csem.Kfor4 e s2 s3 k)); eauto. econstructor; eauto.
+(* break, continue, return 0 *)
+  auto. auto. auto.
+(* return 1 *)
+  rewrite (tr_find_label_expression _ _ _ H0). auto.
+(* switch *)
+  rewrite (tr_find_label_expression _ _ _ H1). apply tr_find_label_ls. auto. constructor; auto.
+(* labeled stmt *)
+  destruct (ident_eq lbl l). exists ts0; exists tk; auto. apply IHs; auto.
+(* goto *)
+  auto.
+
+  induction s; intros; inversion TR; subst; clear TR; simpl.
+(* nil *)
+  auto.
+(* case *)
+  exploit (tr_find_label s (Csem.Kseq (Csem.seq_of_labeled_statement s0) k)); eauto.
+  econstructor; eauto. apply tr_seq_of_labeled_statement; eauto.
+  destruct (Csem.find_label lbl s
+    (Csem.Kseq (Csem.seq_of_labeled_statement s0) k)) as [[s' k'] | ].
+  intros [ts' [tk' [A [B C]]]]. rewrite A. exists ts'; exists tk'; auto.
+  intro EQ. rewrite EQ. eapply IHs; eauto.
+Qed.
 
 End FIND_LABEL.
 
@@ -1020,26 +1589,724 @@ Qed.
 
 (** Forward simulation for expressions. *)
 
+ 
 Lemma tr_val_gen:
   forall le dst v ty a,
   typeof a = ty ->
   (∀ tge e le' m,
       (∀ id, \s id -∗ ⌜ le'!id = le!id ⌝) -∗
-      ⌜ eval_expr tge e le' m a v ⌝) -∗
+                                          ⌜ eval_expr tge e le' m a v ⌝) -∗
   tr_expr le dst (Csyntax.Eval v ty) ((final dst a),a).
 Proof.
-Admitted.
+  intros. destruct dst; simpl; iIntros "HA"; subst; eauto.
+Qed.
+
+Lemma test6_l : forall (P Q : iProp),
+    (P ⊢ P) ->
+    (((P ∧ Q) : iProp) ⊢ P).
+Proof.
+  MonPred.unseal. intros. split. red. intros i h P0. inversion P0. apply H0.
+Qed.
+
+Lemma test6_r : forall (P Q : iProp),
+    (Q ⊢ Q) ->
+    (((P ∧ Q) : iProp) ⊢ Q).
+Proof.
+  MonPred.unseal. intros. split. red. intros i h P0. inversion P0. apply H1.
+Qed.
 
 
 Lemma estep_simulation:
   forall S1 t S2, Cstrategy.estep ge S1 t S2 ->
-  forall S1', match_states S1 S1' ->
-  ∃ S2',
+  forall S1' (MS: match_states S1 S1'),
+  exists S2',
      (plus step1 tge S1' t S2' \/
        (star step1 tge S1' t S2' /\ measure S2 < measure S1)%nat)
   /\ match_states S2 S2'.
 Proof.
+ induction 1; intros; inv MS.
+(* expr *)
+ -  assert (tr_expr le dest r (sl,a) () tmps).
+    + apply soundness2. apply soundness3 in H9. iIntros "HA".
+      iDestruct (H9 with "HA") as "HA". unfold tr_top. iDestruct "HA" as "[HA|%]".
+      iApply "HA". unfold tr_top_val_val in H1. destruct sl; auto.
+      repeat destruct H1. destruct H2. destruct H2. subst. contradiction. contradiction.
+    + exploit tr_simple_rvalue; eauto. apply soundness3 in H1. intro.
+      apply (soundness1 _ tmps). iIntros "HA".
+      iDestruct (H1 with "HA") as "HA". iDestruct (H2 with "HA") as "%".
+      destruct dest.
+      (* for val *)
+      * destruct H3 as (SL1&TY1&EV1). subst sl. iExists _. 
+        iSplit; iPureIntro.
+        -- right; split.
+           ++ apply star_refl.
+           ++ destruct r; simpl; try (contradiction || omega || unfold lt; omega).
+        -- eapply (match_exprstates _ _ _ _ _ _ _ _ _ _ _ ∅); eauto.
+           apply soundness2. iIntros. unfold tr_top. unfold tr_top_val_val. iRight.
+           iPureIntro. exists v. exists (Csyntax.typeof r). split; auto.
+      (* for effects *)
+      * subst sl. iExists _.
+        iSplit; iPureIntro.
+        -- right; split.
+           ++ apply star_refl.
+           ++ destruct r; simpl; try (contradiction || omega || unfold lt; omega).
+        -- econstructor; eauto.
+           instantiate (1 := ∅). apply soundness2.
+           iIntros "HA". unfold tr_top. simpl. iLeft. unfold tr_top_base. simpl.
+           eauto.
+           (* for set *)
+      * inversion H10.
+        (* rval volatile *)
+ - exploit tr_top_leftcontext; eauto.
+   intro. apply soundness3 in H11.
+   apply (soundness1 _ tmps). iIntros "HA". iDestruct (H11 with "HA") as "HA". 
+   iDestruct (H2 with "HA") as "HA". iDestruct ("HA" with "[]") as "HA"; eauto. 
+   iDestruct ("HA" with "[]") as "HA"; eauto.
+   iDestruct "HA" as (dst' sl1 sl2 a') "[P [% R]]".
+   iDestruct "P" as "[HA|%]".
+   + unfold tr_top_base. simpl.
+     iDestruct "HA" as "[_ HA]".
+     iDestruct "HA" as (sla2 sl3) "[HA [HB [HC %]]]".
+     unfold tr_rvalof. rewrite H3. iDestruct "HB" as (t1) "[% HB]".
+     inversion H6. subst.
+     rewrite (surjective_pairing sla2).
+     iDestruct (tr_simple_lvalue with "HA") as "[% [% %]]"; eauto.
+     rewrite H4; simpl. clear H6. iClear "HA". iClear "HC".
+     iExists _. iSplit. 
+     * iPureIntro. left. eapply plus_two. constructor. eapply step_make_set; eauto. traceEq.
+     * iStopProof. apply test3. apply test2.
+       intros. apply test4 in H6. destruct H6 as (tmp0&tmp1&P0&P1&P2&P3). econstructor; eauto.
+       change (final dst' (Etempvar t1 (Csyntax.typeof l)) ++ sl2) with (nil ++ (final dst' (Etempvar t1 (Csyntax.typeof l)) ++ sl2)).
+       apply soundness2. instantiate (1 := tmps0).
+       apply soundness3 in P1. iIntros "HA".
+       rewrite P3. iDestruct (heap_ctx_split with "HA") as "[HA HB]"; eauto.
+       iDestruct (P1 with "HB") as "HB". admit. (* iApply ("HB" with ""). *)    
+         (* -- iApply tr_val_gen; auto. iIntros (? ? ? ?) "HB". *)
+       (*    iDestruct ("HB" with "[HA]")  as "%". *)
+       (*    apply soundness3 in P0. iDestruct (P0 with "HA") as "HA". *)
+       (*    iExists (Csyntax.typeof l). iApply "HA". *)
+       (*    iPureIntro. constructor. rewrite H6. apply Maps.PTree.gss. *)
+       (* -- iIntros. iStopProof. apply test3. apply test2. intros. *)
+       (*    apply Maps.PTree.gso. red. intros. subst. elim H5.  *)
+       (*    iPureIntro. *)
+       (*    apply (soundness1 _ tmps0). iIntros "HA". iDestruct (H6 with "HA") as "[HA [HB [HC HD]]]". *)
+
+   + unfold tr_top_val_val in H5. destruct sl1; auto. destruct H5 as (v'&ty&P0&P1&P2&P3).
+     subst. inversion P3.
+ (* seqand true *)
+ - exploit tr_top_leftcontext; eauto. 
+   intro. apply soundness3 in H9.
+   apply (soundness1 _ tmps). iIntros "HA". iDestruct (H9 with "HA") as "HA". 
+   iDestruct (H2 with "HA") as "HA". iDestruct ("HA" with "[]") as "HA"; eauto.
+   iDestruct ("HA" with "[]") as "HA"; eauto.
+   iDestruct "HA" as (dst' sl1 sl2 a') "[HA [% HB]]". simpl. unfold tr_top.
+   iDestruct "HA" as "[HA|%]".
+   + unfold tr_top_base. simpl. iDestruct "HA" as "[_ HA]". destruct dst'.
+     * simpl. iDestruct "HA" as (sla2 sla3 t0) "[HA [HC [HD %]]]".
+       eapply tr_simple_rvalue in H0.
+       inversion H4. subst.
+       rewrite (surjective_pairing sla2).
+       iDestruct (H0 with "HA") as "[% [% %]]". rewrite H3. simpl. iExists _. iSplit.
+       -- iPureIntro. left. simpl Kseqlist. eapply plus_left. constructor. eapply star_trans.
+          apply step_makeif with (b := true) (v1 := v); auto. congruence.
+          apply push_seq. reflexivity. reflexivity.
+       -- rewrite <- Kseqlist_app. iStopProof. apply test3. apply test2. intros.
+          eapply match_exprstates; eauto.
+          apply soundness2. apply soundness3 in H7. iIntros "HA".
+          iDestruct (H7 with "HA") as "[HA [HB [HC HD]]]".
+          iApply ("HD" with "[HA HB HC]"); eauto.
+          simpl. repeat iSplit; auto. iExists sla3.2. iExists t0. iSplitL "HB". iIntros.
+          rewrite <- surjective_pairing. iApply "HB". iFrame.
+          iSplitL "HC". iFrame. eauto.
+     * simpl. iDestruct "HA" as (sla2 sla3) "[HA [HC %]]".
+       eapply tr_simple_rvalue in H0. rewrite (surjective_pairing sla2).
+       iDestruct (H0 with "HA") as "[% [% %]]". subst. rewrite H5.
+       iExists _. iSplit.
+       -- iPureIntro. left. simpl Kseqlist. eapply plus_left. constructor. eapply star_trans.
+          apply step_makeif with (b := true) (v1 := v); auto. congruence.
+          apply push_seq. reflexivity. reflexivity.
+       -- rewrite <- Kseqlist_app. iStopProof. apply test3. apply test2. intros.
+          eapply match_exprstates; eauto.
+          apply soundness2. apply soundness3 in H3. iIntros "HA".
+          iDestruct (H3 with "HA") as "[HA [HB HC]]".
+          iApply ("HC" with "[HA HB]"); eauto.
+          simpl. iSplitL; eauto. iSplitL "HA"; eauto. iExists sla3.2.
+          rewrite <- surjective_pairing. iApply "HB".
+     * iDestruct "HA" as (sla2 sla3) "[HA [HC [HD %]]]".
+       eapply tr_simple_rvalue in H0. rewrite (surjective_pairing sla2).
+       iDestruct (H0 with "HA") as "[% [% %]]". subst. rewrite H5.
+       iExists _. iSplit.
+       -- iPureIntro. left. simpl Kseqlist. eapply plus_left. constructor. eapply star_trans.
+          apply step_makeif with (b := true) (v1 := v); auto. congruence.
+          apply push_seq. reflexivity. reflexivity.
+       -- rewrite <- Kseqlist_app. iStopProof. apply test3. apply test2. intros.
+          eapply match_exprstates; eauto.
+          apply soundness2. apply soundness3 in H3. iIntros "HA".
+          iDestruct (H3 with "HA") as "[HA [HB [HD HC]]]".
+          iApply ("HC" with "[HA HB HD]"); eauto.
+          simpl. iSplitL; eauto. iSplitL "HA"; eauto. iExists sla3.2. iExists (sd_temp sd).
+          rewrite <- surjective_pairing. iFrame.
+   + unfold tr_top_val_val in H4. destruct sl1; auto. destruct H4 as (v'&ty'&P0&P1&P2&P3).
+     subst. inversion P3.
+     
+ (* seqand false *)
+ - exploit tr_top_leftcontext; intro.
+   apply (soundness1 _ tmps). iIntros "HA". apply soundness3 in H9. iDestruct (H9 with "HA") as "HA".
+   iDestruct (H2 with "HA") as "HA". iDestruct ("HA" with "[]") as "HA"; eauto.
+   iDestruct ("HA" with "[]") as "HA"; eauto.
+   iDestruct "HA" as (dst' sl1 sl2 a') "[P [% R]]".
+   iDestruct "P" as "[[_ HA]|%]".
+   + fold tr_expr. destruct dst'.
+     * iDestruct "HA" as (sla2 sla3 t0) "[HA [HB [HC %]]]". inversion H4; subst.
+       eapply tr_simple_rvalue in H0. rewrite (surjective_pairing sla2).
+       iDestruct (H0 with "HA") as "[% [% %]]". rewrite H3. iExists _. iSplit.
+       -- iPureIntro. left. eapply plus_left. simpl Kseqlist. constructor.
+          eapply star_trans. apply step_makeif with (b := false) (v1 := v); auto. congruence.
+          apply star_one. constructor. constructor. reflexivity. reflexivity.
+       -- iStopProof. apply test3. apply test2. intros. eapply match_exprstates; eauto.
+          change sl2 with (nil ++ sl2). apply soundness3 in H7. apply soundness2.
+          iIntros "HA". iDestruct (H7 with "HA") as "[HA [HB [HC HD]]]".
+          iApply ("HD" with "[HA HB HC]").
+          ++ simpl. iSplitL "HA HB HC"; auto.
+             ** iSplitL "HA" ; eauto. iSplitL; eauto. iIntros "* HA". 
+                iStopProof. apply test3. apply test2. intros.
+                constructor. rewrite H11. apply Maps.PTree.gss.
+          ++ iIntros (? ? ? ?) "HA". iDestruct ("HA" with "[HC]") as "%".
+             iFrame. iStopProof. apply test3. apply test2. intros.
+             constructor. rewrite H11. apply Maps.PTree.gss.
+          ++ iIntros. iPureIntro. apply Maps.PTree.gso. admit.
+          ++ eauto.
+     * iDestruct "HA" as (sla2 sla3) "[HA [HB %]]". simpl in H4. subst.
+       eapply tr_simple_rvalue in H0. rewrite (surjective_pairing sla2).
+       iDestruct (H0 with "HA") as "[% [% %]]". rewrite H3. iExists _. iSplit.
+       -- iPureIntro. left. eapply plus_left. simpl Kseqlist. constructor.
+          apply step_makeif with (b := false) (v1 := v); auto. congruence. reflexivity.
+       -- iStopProof. apply test3. apply test2. intros. eapply match_exprstates; eauto.
+          change sl2 with (nil ++ sl2). apply soundness3 in H6. apply soundness2.
+          iIntros "HA". iDestruct (H6 with "HA") as "[HA [HB HC]]".
+          iApply ("HC" with "[HA HB]"); eauto.
+     * iDestruct "HA" as (sla2 sla3) "[HA [HB [HC %]]]". simpl in *. subst.
+       eapply tr_simple_rvalue in H0. rewrite (surjective_pairing sla2).
+       iDestruct (H0 with "HA") as "[% [% %]]". rewrite H3. iExists _. iSplit.
+       -- iPureIntro. left. eapply plus_left. simpl Kseqlist. constructor.
+          eapply star_trans. apply step_makeif with (b := false) (v1 := v); auto. congruence.
+          apply push_seq. reflexivity. reflexivity.
+       --  rewrite <- Kseqlist_app.
+           iStopProof. apply test3. apply test2. intros. eapply match_exprstates; eauto.
+           apply soundness3 in H6. apply soundness2.
+          iIntros "HA". iDestruct (H6 with "HA") as "[HA [HB [HC HD]]]".
+          iApply ("HD" with "[HA HB HC]"). simpl. iSplitL "HA"; auto.
+          iExists (Econst_int Int.zero ty).
+          iSplit; eauto.
+          ++ iIntros (? ? ? ?) "HA". iDestruct ("HA" with "[HC]") as "%".
+             iFrame. iPureIntro.
+             econstructor; eauto.
+          ++ iIntros. eauto.
+          ++ eauto.
+   + unfold tr_top_val_val in H4. destruct sl1; auto. destruct H4 as (v'&ty0&P0&P1&P2&P3).
+     subst. inversion P3.
+ (* seqor true *)
+ - exploit tr_top_leftcontext. intro. apply soundness3 in H9.
+   apply (soundness1 _ tmps). iIntros "HA". iDestruct (H9 with "HA") as "HA". 
+   iDestruct (H2 with "HA") as "HA". iDestruct ("HA" with "[]") as "HA"; eauto.
+   iDestruct ("HA" with "[]") as "HA"; eauto.
+   iDestruct "HA" as (dst' sl1 sl2 a') "[HA [% HB]]". simpl. unfold tr_top.
+   iDestruct "HA" as "[[_ HA]|%]".
+   + unfold tr_top_base. fold tr_expr. simpl. destruct dst'.
+     * iDestruct "HA" as (sla2 sla3 t0) "[HA [HD [HC %]]]". inversion H4; subst.
+       eapply tr_simple_rvalue in H0. rewrite (surjective_pairing sla2).
+       iDestruct (H0 with "HA") as "[% [% %]]". rewrite H3. iExists _. iSplit.
+       -- iPureIntro. left. eapply plus_left. simpl Kseqlist. constructor.
+          eapply star_trans. apply step_makeif with (b := true) (v1 := v); auto. congruence.
+          apply star_one. constructor. constructor. reflexivity. reflexivity.
+       -- iStopProof. apply test3. apply test2. intros. eapply match_exprstates; eauto.
+          change sl2 with (nil ++ sl2). apply soundness3 in H7. apply soundness2.
+          iIntros "HA". iDestruct (H7 with "HA") as "[HA [HB [HC HD]]]".
+          iApply ("HD" with "[HA HB HC]"). simpl. iSplitL "HA"; auto.
+          iSplit; eauto.
+          ++ iIntros (? ? ? ?) "HA". iDestruct ("HA" with "[HC]") as "%".
+             iFrame. iStopProof. apply test3. apply test2. intros.
+             constructor. rewrite H11. apply Maps.PTree.gss.
+          ++ iIntros. iPureIntro. apply Maps.PTree.gso. admit.
+          ++ eauto.
+     * iDestruct "HA" as (sla2 sla3) "[HA [HC %]]". simpl in H4. subst.
+       eapply tr_simple_rvalue in H0. rewrite (surjective_pairing sla2).
+       iDestruct (H0 with "HA") as "[% [% %]]". rewrite H3. iExists _. iSplit.
+       -- iPureIntro. left. eapply plus_left. simpl Kseqlist. constructor.
+          apply step_makeif with (b := true) (v1 := v); auto. congruence. reflexivity.
+       -- iStopProof. apply test3. apply test2. intros. eapply match_exprstates; eauto.
+          change sl2 with (nil ++ sl2). apply soundness3 in H6. apply soundness2.
+          iIntros "HA". iDestruct (H6 with "HA") as "[HA [HB HC]]".
+          iApply ("HC" with "[HA HB]"); eauto.
+     * iDestruct "HA" as (sla2 sla3) "[HA [HD [HC %]]]". simpl in *. subst.
+       eapply tr_simple_rvalue in H0. rewrite (surjective_pairing sla2).
+       iDestruct (H0 with "HA") as "[% [% %]]". rewrite H3. iExists _. iSplit.
+       -- iPureIntro. left. eapply plus_left. simpl Kseqlist. constructor.
+          eapply star_trans. apply step_makeif with (b := true) (v1 := v); auto. congruence.
+          apply push_seq. reflexivity. reflexivity.
+       --  rewrite <- Kseqlist_app.
+           iStopProof. apply test3. apply test2. intros. eapply match_exprstates; eauto.
+           apply soundness3 in H6. apply soundness2.
+           iIntros "HA". iDestruct (H6 with "HA") as "[HA [HB [HC HD]]]".
+           iApply ("HD" with "[HA HB HC]"). simpl. iSplitL "HA"; auto.
+           iExists (Econst_int Int.one ty).
+           iSplit; eauto.
+           ++ iIntros (? ? ? ?) "HA". iDestruct ("HA" with "[HC]") as "%".
+              iFrame. iPureIntro.
+              econstructor; eauto.
+           ++ iIntros. eauto.
+           ++ eauto.
+   + unfold tr_top_val_val in H4. destruct sl1; auto. destruct H4 as (v'&ty0&P0&P1&P2&P3).
+     subst. inversion P3.
+     
+ (* seqor false *)
+ - exploit tr_top_leftcontext. intro. apply soundness3 in H9.
+   apply (soundness1 _ tmps). iIntros "HA". iDestruct (H9 with "HA") as "HA". 
+   iDestruct (H2 with "HA") as "HA". iDestruct ("HA" with "[]") as "HA"; eauto.
+   iDestruct ("HA" with "[]") as "HA"; eauto.
+   iDestruct "HA" as (dst' sl1 sl2 a') "[HA [% HB]]". simpl. unfold tr_top.
+   iDestruct "HA" as "[[_ HA]|%]".
+   + fold tr_expr. unfold tr_top_base.  simpl. destruct dst'.
+     * iDestruct "HA" as (sla2 sla3 t0) "[HA [HD [HC %]]]". inversion H4; subst.
+       eapply tr_simple_rvalue in H0. rewrite (surjective_pairing sla2).
+       iDestruct (H0 with "HA") as "[% [% %]]". rewrite H3. iExists _. iSplit.
+       -- iPureIntro. left. eapply plus_left. simpl Kseqlist. constructor.
+          eapply star_trans. apply step_makeif with (b := false) (v1 := v); auto. congruence.
+          apply push_seq. constructor. constructor. 
+       -- rewrite <- Kseqlist_app.
+          iStopProof. apply test3. apply test2. intros. eapply match_exprstates; eauto.
+          apply soundness3 in H7. apply soundness2.
+          iIntros "HA". iDestruct (H7 with "HA") as "[HA [HB [HC HD]]]".
+          iApply ("HD" with "[HA HB HC]"). simpl. iSplitL "HA"; auto. iExists sla3.2.
+          iExists t0.
+          ++ rewrite <- surjective_pairing. iFrame. eauto.
+          ++ eauto.
+          ++ eauto.
+     * iDestruct "HA" as (sla2 sla3) "[HA [HC %]]". simpl in H4. subst.
+       eapply tr_simple_rvalue in H0. rewrite (surjective_pairing sla2).
+       iDestruct (H0 with "HA") as "[% [% %]]". rewrite H3. iExists _. iSplit.
+       -- iPureIntro. left. eapply plus_left. simpl Kseqlist. constructor.
+          eapply star_trans.
+          apply step_makeif with (b := false) (v1 := v); auto. congruence. apply push_seq.
+          reflexivity. reflexivity.
+       -- rewrite <- Kseqlist_app.
+          iStopProof. apply test3. apply test2. intros. eapply match_exprstates; eauto.
+          apply soundness3 in H6. apply soundness2.
+          iIntros "HA". iDestruct (H6 with "HA") as "[HA [HB HC]]".
+          iApply ("HC" with "[HA HB]"); eauto. simpl. iSplitL "HA"; eauto.
+          iExists sla3.2. rewrite <- surjective_pairing. iApply "HB".
+     * iDestruct "HA" as (sla2 sla3) "[HA [HD [HC %]]]". simpl in *. subst.
+       eapply tr_simple_rvalue in H0. rewrite (surjective_pairing sla2).
+       iDestruct (H0 with "HA") as "[% [% %]]". rewrite H3. iExists _. iSplit.
+       -- iPureIntro. left. eapply plus_left. simpl Kseqlist. constructor.
+          eapply star_trans. apply step_makeif with (b := false) (v1 := v); auto. congruence.
+          apply push_seq. reflexivity. reflexivity.
+       --  rewrite <- Kseqlist_app.
+           iStopProof. apply test3. apply test2. intros. eapply match_exprstates; eauto.
+           apply soundness3 in H6. apply soundness2.
+           iIntros "HA". iDestruct (H6 with "HA") as "[HA [HB [HC HD]]]".
+           iApply ("HD" with "[HA HB HC]"); eauto. simpl. iSplitL "HA"; auto.
+           iExists sla3.2. iExists (sd_temp sd). rewrite <- surjective_pairing. iFrame.
+   + unfold tr_top_val_val in H4. destruct sl1; auto. destruct H4 as (v'&ty0&P0&P1&P2&P3).
+     subst. inversion P3.
+     
+     (* condition *)
+  - exploit tr_top_leftcontext. intro. apply soundness3 in H9.
+   apply (soundness1 _ tmps). iIntros "HA". iDestruct (H9 with "HA") as "HA". 
+   iDestruct (H2 with "HA") as "HA". iDestruct ("HA" with "[]") as "HA"; eauto.
+   iDestruct ("HA" with "[]") as "HA"; eauto.
+   iDestruct "HA" as (dst' sl1 sl2 a') "[HA [% HB]]". simpl. unfold tr_top.
+   iDestruct "HA" as "[[_ HA]|%]".
+   + fold tr_expr. unfold tr_top_base.  simpl. destruct dst'.
+     * iDestruct "HA" as (sla2 sla3 sla4 t0) "[HA [HD [HC %]]]".
+       (* iDestruct ("HC" with "HD") as "HC". *)
+       inversion H4; subst.
+       eapply tr_simple_rvalue in H0. rewrite (surjective_pairing sla2).
+       iDestruct (H0 with "HA") as "[% [% %]]". rewrite H3; simpl Kseqlist. destruct b. 
+       -- iExists _. iSplit.
+          ++ iPureIntro. left. eapply plus_left. constructor.
+             eapply star_trans. apply step_makeif with (b := true) (v1 := v); auto. congruence.
+             apply push_seq. reflexivity. reflexivity.
+          ++ rewrite <- Kseqlist_app.
+             iStopProof. apply test3. apply test2. intros. eapply match_exprstates; eauto.
+             apply soundness3 in H7. apply soundness2.
+             iIntros "HA". iDestruct (H7 with "HA") as "[HA [HB [HC HD]]]".
+             iApply ("HD" with "[HA HB HC]"); eauto. simpl. iSplitL "HA"; auto. iExists sla3.2.
+             iExists t0. iSplitL "HC"; eauto.
+             rewrite <- surjective_pairing. iIntros "HB".
+             iDestruct ("HC" with "HB") as "HA". iStopProof. apply test6_l. eauto.
+       -- iExists _. iSplit.
+          ++ iPureIntro. left. eapply plus_left. constructor.
+             eapply star_trans. apply step_makeif with (b := false) (v1 := v); auto. congruence.
+             apply push_seq. reflexivity. reflexivity.
+          ++ rewrite <- Kseqlist_app.
+             iStopProof. apply test3. apply test2. intros. eapply match_exprstates; eauto.
+             apply soundness3 in H7. apply soundness2.
+             iIntros "HA". iDestruct (H7 with "HA") as "[HA [HB [HC HD]]]".
+             iApply ("HD" with "[HA HB HC]"); eauto. simpl. iSplitL "HA"; eauto. iExists sla4.2.
+             iExists t0. rewrite <- surjective_pairing. iFrame. iSplitL; eauto.
+             iIntros "HA". iDestruct ("HC" with "HA") as "HA". iStopProof. apply test6_r. eauto.
+     * iDestruct "HA" as (sla2 sla3 sl4) "[HA [HC [HD %]]]". subst.
+       eapply tr_simple_rvalue in H0. rewrite (surjective_pairing sla2).
+       iDestruct (H0 with "HA") as "[% [% %]]". rewrite H3; simpl Kseqlist. destruct b.
+       -- iExists _. iSplit.
+          ++ iPureIntro. left. eapply plus_left. constructor.
+             eapply star_trans. apply step_makeif with (b := true) (v1 := v); auto. congruence.
+             apply push_seq. reflexivity. traceEq.
+          ++ rewrite <- Kseqlist_app.
+             iStopProof. apply test3. apply test2. intros. econstructor; eauto.
+             apply soundness3 in H6. apply soundness2.
+             iIntros "HA". iDestruct (H6 with "HA") as "[HA [HB [HC HD]]]".
+             iApply ("HD" with "[HA HB HC]"); eauto. simpl. iSplitL "HA HC"; eauto.
+             iExists sla3.2. rewrite <- surjective_pairing. iFrame.
+       -- iExists _. iSplit.
+          ++ iPureIntro. left. eapply plus_left. constructor.
+             eapply star_trans. apply step_makeif with (b := false) (v1 := v); auto. congruence.
+             apply push_seq. reflexivity. traceEq.
+          ++ rewrite <- Kseqlist_app.
+             iStopProof. apply test3. apply test2. intros. econstructor; eauto.
+             apply soundness3 in H6. apply soundness2.
+             iIntros "HA". iDestruct (H6 with "HA") as "[HA [HB [HC HD]]]".
+             iApply ("HD" with "[HA HB HC]"); eauto. simpl. iSplitL "HA HB"; eauto.
+             iExists sl4.2. rewrite <- surjective_pairing. iFrame.
+     * iDestruct "HA" as (sla2 sla3 sla4 t0) "[HA [HD [HC %]]]". subst.
+       eapply tr_simple_rvalue in H0. rewrite (surjective_pairing sla2).
+       iDestruct (H0 with "HA") as "[% [% %]]". rewrite H3. destruct b.
+       -- iExists _. iSplit.
+          ++ iPureIntro.  left. eapply plus_left. constructor. simpl.
+             eapply star_trans. apply step_makeif with (b := true) (v1 := v); auto. congruence.
+             apply push_seq. reflexivity. traceEq.
+          ++ rewrite <- Kseqlist_app.
+             iStopProof. apply test3. apply test2. intros. econstructor; eauto.
+             apply soundness3 in H6. apply soundness2.
+             iIntros "HA". iDestruct (H6 with "HA") as "[HA [HB [HC HD]]]".
+             iApply ("HD" with "[HA HB HC]"); eauto. simpl. iSplitL "HA"; auto.
+             iExists sla3.2. iExists t0. rewrite <- surjective_pairing. iFrame.
+             iIntros "HA". iDestruct ("HC" with "HA") as "HA". iStopProof. apply test6_l. eauto.
+       -- iExists _. iSplit.
+          ++ iPureIntro. left. eapply plus_left. constructor. simpl.
+             eapply star_trans. apply step_makeif with (b := false) (v1 := v); auto. congruence.
+             apply push_seq. reflexivity. traceEq.
+          ++ rewrite <- Kseqlist_app.
+             iStopProof. apply test3. apply test2. intros. econstructor; eauto.
+             apply soundness3 in H6. apply soundness2.
+             iIntros "HA". iDestruct (H6 with "HA") as "[HA [HB [HC HD]]]".
+             iApply ("HD" with "[HA HB HC]"); eauto. simpl. iSplitL "HA"; auto.
+             iExists sla4.2. iExists t0. rewrite <- surjective_pairing. iFrame. iIntros "HA".
+             iDestruct ("HC" with "HA") as "HA". iStopProof. apply test6_r. eauto.
+   + unfold tr_top_val_val in H4. destruct sl1; auto. destruct H4 as (v'&ty0&P0&P1&P2&P3).
+     subst. inversion P3.
+     
+  (* assign *)
+  - exploit tr_top_leftcontext. intro. apply soundness3 in H12.
+    apply (soundness1 _ tmps). iIntros "HA". iDestruct (H12 with "HA") as "HA". 
+    iDestruct (H4 with "HA") as "HA". iDestruct ("HA" with "[]") as "HA"; eauto.
+    iDestruct ("HA" with "[]") as "HA"; eauto.
+    iDestruct "HA" as (dst' sl1 sl2 a') "[HA [% HB]]". simpl. unfold tr_top.
+    iDestruct "HA" as "[[_ HA]|%]"; fold tr_expr. 
+    + iDestruct "HA" as (sla2 sla3) "[HA [HC HD]]".
+      destruct dst'; iDestruct "HD" as "[[% %]| HD]"; try discriminate.
+      * admit.  (* Toujours (forall id, In id tmps -> le ! id = le' ! id *)
+      * simpl in *. subst. clear H7.
+        eapply tr_simple_lvalue in H0.
+        eapply tr_simple_rvalue in H1. rewrite (surjective_pairing sla2).
+        rewrite (surjective_pairing sla3).
+        iDestruct (H0 with "HA") as "[% [% %]]". 
+        iDestruct (H1 with "HC") as "[% [% %]]". rewrite H5. rewrite H8. simpl Kseqlist.
+        iExists _. iSplit.
+        -- iPureIntro. left. eapply plus_left. constructor.
+           apply star_one. eapply step_make_assign; eauto.
+           rewrite <- H9; eauto. traceEq.
+        -- iStopProof. apply test3. apply test2. intros. econstructor; eauto.
+           apply soundness3 in H14. apply soundness2.
+           iIntros "HA". iDestruct (H14 with "HA") as "[HA [HB HC]]".
+           change sl2 with (nil ++ sl2).
+           iApply ("HC" with "[HA HB]"); eauto.
+      * admit.
+      * admit.
+    + unfold tr_top_val_val in H6. destruct sl1; auto. destruct H6 as (v''&ty0&P0&P1&P2&P3).
+      inversion P3.
+
+  (* assignop *)
+  - exploit tr_top_leftcontext. intro. apply soundness3 in H15.
+    apply (soundness1 _ tmps). iIntros "HA". iDestruct (H15 with "HA") as "HA". 
+    iDestruct (H6 with "HA") as "HA". iDestruct ("HA" with "[]") as "HA"; eauto.
+    iDestruct ("HA" with "[]") as "HA"; eauto.
+    iDestruct "HA" as (dst' sl1 sl2 a') "[HA [% HB]]". simpl. unfold tr_top.
+    iDestruct "HA" as "[[_ HA]|%]"; fold tr_expr. 
+    + iDestruct "HA" as (sla2 sla3 sla4) "[HA [HC [HD HE]]]".
+      destruct dst'; iDestruct "HE" as "[[% %]| HE]"; try discriminate.
+      * admit.  (* Toujours (forall id, In id tmps -> le ! id = le' ! id *)
+      * admit.
+      * admit.
+      * admit.
+    + unfold tr_top_val_val in H8. destruct sl1; auto. destruct H8 as (v''&ty0&P0&P1&P2&P3).
+      inversion P3.
+
+  (* assignop stuck *)
+  - exploit tr_top_leftcontext; intro. apply soundness3 in H12.
+    apply (soundness1 _ tmps). iIntros "HA". iDestruct (H12 with "HA") as "HA". 
+    iDestruct (H4 with "HA") as "HA". iDestruct ("HA" with "[]") as "HA"; eauto.
+    iDestruct ("HA" with "[]") as "HA"; eauto.
+    iDestruct "HA" as (dst' sl1 sl2 a') "[HA [% HB]]". simpl. unfold tr_top.
+    iDestruct "HA" as "[[_ HA]|%]"; fold tr_expr. 
+    + iDestruct "HA" as (sla2 sla3 sla4) "[HA [HC [HD HE]]]".
+      destruct dst'; iDestruct "HE" as "[[% %]| HE]"; try discriminate.
+      * iDestruct "HE" as (t1) "[HE %]". inversion H6; subst.
+        eapply tr_simple_lvalue in H0. rewrite (surjective_pairing sla2).
+        iDestruct (H0 with "HA") as "[% [% %]]".
+        eapply tr_simple_rvalue in H2. rewrite (surjective_pairing sla3).
+        iDestruct (H2 with "HC") as "[% [% %]]".
+        eapply step_tr_rvalof in H1. rewrite (surjective_pairing sla4).
+        iDestruct (H1 with "HD") as "HD".
+        iDestruct ("HD" with "[]") as (le') "[[% [% %]] HD]"; eauto. rewrite H5. rewrite H9.
+        simpl Kseqlist. iExists _. iSplit.
+        -- iPureIntro. right; split. rewrite app_ass. rewrite Kseqlist_app. eexact H15.
+           simpl. unfold lt; omega.
+        -- iPureIntro. constructor.
+        -- eauto.
+      * simpl in *. subst. clear H6.
+        eapply tr_simple_lvalue in H0. rewrite (surjective_pairing sla2).
+        iDestruct (H0 with "HA") as "[% [% %]]".
+        eapply tr_simple_rvalue in H2. rewrite (surjective_pairing sla3).
+        iDestruct (H2 with "HC") as "[% [% %]]".
+        eapply step_tr_rvalof in H1. rewrite (surjective_pairing sla4).
+        iDestruct (H1 with "HD") as "HD".
+        iDestruct ("HD" with "[]") as (le') "[[% [% %]] HD]"; eauto. rewrite H5. rewrite H8.
+        simpl Kseqlist. iExists _. iSplit.
+        -- iPureIntro. right; split. rewrite app_ass. rewrite Kseqlist_app. eexact H14.
+           simpl. unfold lt. omega.
+        -- iPureIntro. constructor.
+        -- auto.
+      * iDestruct "HE" as (t1) "[HE %]". inversion H6; subst.
+        eapply tr_simple_lvalue in H0. rewrite (surjective_pairing sla2).
+        iDestruct (H0 with "HA") as "[% [% %]]".
+        eapply tr_simple_rvalue in H2. rewrite (surjective_pairing sla3).
+        iDestruct (H2 with "HC") as "[% [% %]]".
+        eapply step_tr_rvalof in H1. rewrite (surjective_pairing sla4).
+        iDestruct (H1 with "HD") as "HD".
+        iDestruct ("HD" with "[]") as (le') "[[% [% %]] HD]"; eauto. rewrite H5. rewrite H9.
+        simpl Kseqlist. iExists _. iSplit.
+        -- iPureIntro. right; split. rewrite app_ass. rewrite Kseqlist_app. eexact H15.
+           simpl. unfold lt; omega.
+        -- iPureIntro. constructor.
+        -- eauto.
+      * iDestruct "HE" as (t1) "[HE %]". inversion H6; subst.
+        eapply tr_simple_lvalue in H0. rewrite (surjective_pairing sla2).
+        iDestruct (H0 with "HA") as "[% [% %]]".
+        eapply tr_simple_rvalue in H2. rewrite (surjective_pairing sla3).
+        iDestruct (H2 with "HC") as "[% [% %]]".
+        eapply step_tr_rvalof in H1. rewrite (surjective_pairing sla4).
+        iDestruct (H1 with "HD") as "HD".
+        iDestruct ("HD" with "[]") as (le') "[[% [% %]] HD]"; eauto. rewrite H5. rewrite H9.
+        simpl Kseqlist. iExists _. iSplit.
+        -- iPureIntro. right; split. rewrite app_ass. rewrite Kseqlist_app. eexact H15.
+           simpl. unfold lt; omega.
+        -- iPureIntro. constructor.
+        -- eauto.
+    + unfold tr_top_val_val in H6. destruct sl1; auto. destruct H6 as (v'&ty0&P0&P1&P2&P3).
+      inversion P3.
+
+  (* postincr *)
+  - exploit tr_top_leftcontext; intro. apply soundness3 in H14.
+    apply (soundness1 _ tmps). iIntros "HA". iDestruct (H14 with "HA") as "HA". 
+    iDestruct (H5 with "HA") as "HA". iDestruct ("HA" with "[]") as "HA"; eauto.
+    iDestruct ("HA" with "[]") as "HA"; eauto.
+    iDestruct "HA" as (dst' sl1 sl2 a') "[HA [% HB]]". simpl. unfold tr_top.
+    iDestruct "HA" as "[[_ HA]|%]"; fold tr_expr. 
+    + iDestruct "HA" as "[HA| HA]".
+      * admit.
+      * admit.
+    + unfold tr_top_val_val in H7. destruct sl1; try contradiction.
+      destruct H7 as (v&ty&P0&P1&P2&P3). inversion P3.
+
+  (* postincr stuck *)
+  - exploit tr_top_leftcontext; intro. apply soundness3 in H11.
+    apply (soundness1 _ tmps). iIntros "HA". iDestruct (H11 with "HA") as "HA". 
+    iDestruct (H3 with "HA") as "HA". iDestruct ("HA" with "[]") as "HA"; eauto.
+    iDestruct ("HA" with "[]") as "HA"; eauto.
+    iDestruct "HA" as (dst' sl1 sl2 a') "[HA [% HB]]". simpl. unfold tr_top.
+    iDestruct "HA" as "[[_ HA]|%]"; fold tr_expr. 
+    + iDestruct "HA" as "[HA|HA]".
+      * iDestruct "HA" as (sla2 sla3) "[HA [HC %]]".
+        eapply tr_simple_lvalue in H0. rewrite (surjective_pairing sla2).
+        iDestruct (H0 with "HA") as "[% [% %]]".
+        subst. 
+        eapply step_tr_rvalof in H1; eauto. rewrite (surjective_pairing sla3).
+        iDestruct (H1 with "HC") as "HC".
+        iDestruct ("HC" with "[]") as (le') "[[% [% %]] HC]"; eauto. simpl in *. rewrite H5.
+        rewrite H6. simpl Kseqlist.
+        iExists _. iSplit; iPureIntro.
+        -- right; split. rewrite app_ass; rewrite Kseqlist_app. eexact H4.
+           unfold lt. omega.
+        -- constructor.
+      * iDestruct "HA" as (sla2 t1) "[HA [HC %]]". inversion H5. subst. 
+        eapply tr_simple_lvalue in H0. rewrite (surjective_pairing sla2).
+        iDestruct (H0 with "HA") as "[% [% %]]".
+        rewrite H4. simpl Kseqlist. iExists _. iSplit.
+        -- iPureIntro. left. eapply plus_two. constructor. eapply step_make_set; eauto.
+           traceEq.
+        -- iPureIntro. constructor.
+    + unfold tr_top_val_val in H5. destruct sl1; auto. destruct H5 as (v'&ty0&P0&P1&P2&P3).
+      inversion P3.
+
+  (* comma *)
+  - exploit tr_top_leftcontext; intro. apply soundness3 in H9.
+    apply (soundness1 _ tmps). iIntros "HA". iDestruct (H9 with "HA") as "HA". 
+    iDestruct (H1 with "HA") as "HA". iDestruct ("HA" with "[]") as "HA"; eauto.
+    iDestruct ("HA" with "[]") as "HA"; eauto.
+    iDestruct "HA" as (dst' sl1 sl2 a') "[HA [% HB]]". simpl. unfold tr_top.
+    iDestruct "HA" as "[[_ HA]|%]"; fold tr_expr. 
+    + iDestruct "HA" as (sla2 sl3) "[HA [HD [HC %]]]". simpl in *. subst.
+      eapply tr_simple_rvalue in H0. rewrite (surjective_pairing sla2).
+      iDestruct (H0 with "HA") as "%". rewrite H2. simpl Kseqlist. iClear "HA".
+      iExists _. iSplit.
+      * iPureIntro. right; split. apply star_refl. simpl. apply plus_lt_compat_r.
+        apply (leftcontext_size _ _ _ H). simpl. omega.
+      * iStopProof. apply test3. apply test2. intros. econstructor; eauto.
+        apply soundness3 in H3. apply soundness2.
+        iIntros "HA". iDestruct (H3 with "HA") as "[HB [HC HD]]".
+        iApply ("HD" with "[HB HC]"); eauto. iApply "HB". iFrame.
+    + unfold tr_top_val_val in H3. destruct sl1; auto. destruct H3 as (v'&ty0&P0&P1&P2&P3).
+      inversion P3.
+
+  (* paren *)
+  - exploit tr_top_leftcontext; intro. apply soundness3 in H9.
+    apply (soundness1 _ tmps). iIntros "HA". iDestruct (H9 with "HA") as "HA". 
+    iDestruct (H2 with "HA") as "HA". iDestruct ("HA" with "[]") as "HA"; eauto.
+    iDestruct ("HA" with "[]") as "HA"; eauto.
+    iDestruct "HA" as (dst' sl1 sl2 a') "[HA [% HB]]". simpl. unfold tr_top.
+    iDestruct "HA" as "[[_ HA]|%]"; fold tr_expr. 
+    + destruct dst'.
+      * iDestruct "HA" as (a2 t0) "[HA [HC %]]".
+        eapply tr_simple_rvalue in H0. iDestruct ("HA" with "HC") as "HA".
+        iDestruct (H0 with "HA") as (?) "[% [% %]]". simpl in *. subst. simpl Kseqlist.
+        iExists _. iSplit.
+        -- iPureIntro. left. eapply plus_left. constructor. apply star_one. econstructor.
+           econstructor; eauto. rewrite <- H7; eauto. traceEq.
+        -- admit.
+      * iDestruct "HA" as (a2) "HA".
+        eapply tr_simple_rvalue in H0. simpl.
+        iDestruct (H0 with "HA") as "%". simpl in *. subst. simpl Kseqlist.
+        iExists _. iSplit.
+        -- iPureIntro. right; split. apply star_refl. simpl. apply plus_lt_compat_r.
+           apply (leftcontext_size _ _ _ H). simpl.
+           unfold lt. apply le_n_S. apply le_0_n.
+        -- iStopProof. apply test3. apply test2. intros. econstructor; eauto.
+           apply soundness3 in H3. apply soundness2.
+           iIntros "HA". iDestruct (H3 with "HA") as "[HA HB]".
+           change sl2 with (nil ++ sl2).
+           iApply ("HB" with "[HA]"); eauto.
+      * admit.
+    + unfold tr_top_val_val in H4. destruct sl1; auto. destruct H4 as (v'&ty0&P0&P1&P2&P3).
+      inversion P3.
+
+  (* call *)
+  - exploit tr_top_leftcontext; intro. apply soundness3 in H12.
+    apply (soundness1 _ tmps). iIntros "HA". iDestruct (H12 with "HA") as "HA". 
+    iDestruct (H5 with "HA") as "HA". iDestruct ("HA" with "[]") as "HA"; eauto.
+    iDestruct ("HA" with "[]") as "HA"; eauto.
+    iDestruct "HA" as (dst' sl1 sl2 a') "[HA [% HB]]". simpl. unfold tr_top.
+    iDestruct "HA" as "[[_ HA]|%]"; fold tr_expr; fold tr_exprlist.
+    + destruct dst'.
+      * iDestruct "HA" as (sla2 slal3 t0) "[HA [HC [HD [_ %]]]]". inversion H7; subst.
+        eapply tr_simple_rvalue in H1. rewrite (surjective_pairing sla2).
+        iDestruct (H1 with "HA") as "[% [% %]]". rewrite H6.
+        rewrite (surjective_pairing slal3).
+        iDestruct (tr_simple_exprlist with "HC") as "HC"; eauto.
+        iDestruct ("HC" with "[]") as "[% %]"; eauto. rewrite H10. simpl Kseqlist.
+        apply functions_translated in H3. destruct H3 as (tf'&P0&P1).
+        iExists _. iSplit.
+        -- iPureIntro. left. eapply plus_left. constructor. apply star_one.
+           econstructor; eauto. rewrite <- H8; eauto. exploit type_of_fundef_preserved; eauto.
+           congruence. traceEq.
+        -- iStopProof. apply test3. apply test2. intros. constructor; auto.
+           econstructor; eauto. intros.
+           apply soundness3 in H3. apply soundness2.
+           iIntros "HA". iDestruct (H3 with "HA") as "[HA [HB HC]]".
+           change sl2 with (nil ++ sl2).
+           iApply ("HC" with "[HA HB]"); eauto. simpl. iSplitL "HA"; eauto.
+           iSplit; eauto. iIntros (? ? ? ?) "HA".
+           iDestruct ("HA" with "HB") as "%". iPureIntro. constructor. rewrite H15.
+           apply Maps.PTree.gss. iIntros. admit.
+      * iDestruct "HA" as (sla2 slal3) "[HA [HC %]]". simpl in *. subst.
+        eapply tr_simple_rvalue in H1. rewrite (surjective_pairing sla2).
+        iDestruct (H1 with "HA") as "[% [% %]]". rewrite H6.
+        rewrite (surjective_pairing slal3).
+        iDestruct (tr_simple_exprlist with "HC") as "HC"; eauto.
+        iDestruct ("HC" with "[]") as "[% %]"; eauto. rewrite H9. simpl Kseqlist.
+        apply functions_translated in H3. destruct H3 as (tf'&P0&P1).
+        iExists _. iSplit.
+        -- iPureIntro. left. eapply plus_left. constructor. apply star_one.
+           econstructor; eauto. rewrite <- H7; eauto. exploit type_of_fundef_preserved; eauto.
+           congruence. traceEq.
+        -- iStopProof. apply test3. apply test2. intros. constructor; auto.
+           econstructor; eauto. intros.
+           apply soundness3 in H3. apply soundness2.
+           iIntros "HA". iDestruct (H3 with "HA") as "[HA HB]".
+           change sl2 with (nil ++ sl2).
+           iApply ("HB" with "[HA]"); eauto.
+      * admit.
+    + unfold tr_top_val_val in H7. destruct sl1; auto. destruct H7 as (v'&ty0&P0&P1&P2&P3).
+      inversion P3.
+
+  (* builtin *)
+  - exploit tr_top_leftcontext; intro. apply soundness3 in H9.
+    apply (soundness1 _ tmps). iIntros "HA". iDestruct (H9 with "HA") as "HA". 
+    iDestruct (H2 with "HA") as "HA". iDestruct ("HA" with "[]") as "HA"; eauto.
+    iDestruct ("HA" with "[]") as "HA"; eauto.
+    iDestruct "HA" as (dst' sl1 sl2 a') "[HA [% HB]]". simpl. unfold tr_top.
+    iDestruct "HA" as "[[_ HA]|%]"; fold tr_expr; fold tr_exprlist.
+    + destruct dst'.
+      * iDestruct "HA" as (slal2 t1) "[HA [HD [_ %]]]". inversion H4; subst.
+        rewrite (surjective_pairing slal2).
+        iDestruct (tr_simple_exprlist with "HA") as "HA"; eauto.
+        iDestruct ("HA" with "[]") as "[% %]"; eauto. rewrite H3. simpl Kseqlist.
+        iExists _. iSplit.
+        -- iPureIntro. left. eapply plus_left. constructor. apply star_one.
+           econstructor; eauto. eapply external_call_symbols_preserved; eauto. apply senv_preserved.
+           traceEq.
+        -- iStopProof. apply test3. apply test2. intros. econstructor; eauto.
+           apply soundness3 in H6. apply soundness2.
+           iIntros "HA". iDestruct (H6 with "HA") as "[HA HB]".
+           change sl2 with (nil ++ sl2).
+           iApply ("HB" with "[HA]"); eauto. epose tr_val_gen.
+           change [] with (final For_val (Etempvar t1 ty)).
+           iApply tr_val_gen. reflexivity. iIntros. admit. admit.
+      * iDestruct "HA" as (slal2) "[HA %]". simpl in *; subst.
+        rewrite (surjective_pairing slal2).
+        iDestruct (tr_simple_exprlist with "HA") as "HA"; eauto.
+        iDestruct ("HA" with "[]") as "[% %]"; eauto. rewrite H3. simpl Kseqlist.
+        iExists _. iSplit.
+        -- iPureIntro. left. eapply plus_left. constructor. apply star_one.
+           econstructor; eauto. eapply external_call_symbols_preserved; eauto. apply senv_preserved.
+           traceEq.
+        -- iStopProof. apply test3. apply test2. intros. econstructor; eauto.
+           apply soundness3 in H5. apply soundness2.
+           iIntros "HA". iDestruct (H5 with "HA") as "HA".
+           change sl2 with (nil ++ sl2). iApply "HA"; eauto.
+      * iDestruct "HA" as (slal2 t1) "[HA [HD [HE %]]]". inversion H4; subst.
+        rewrite (surjective_pairing slal2).
+        iDestruct (tr_simple_exprlist with "HA") as "HA"; eauto.
+        iDestruct ("HA" with "[]") as "[% %]"; eauto. rewrite H3. simpl Kseqlist.
+        iExists _. iSplit.
+        -- iPureIntro. left. eapply plus_left. constructor. apply star_one.
+           econstructor; eauto. eapply external_call_symbols_preserved; eauto. apply senv_preserved.
+           traceEq.
+        -- iStopProof. apply test3. apply test2. intros. econstructor; eauto.
+           apply soundness3 in H6. apply soundness2.
+           iIntros "HA". iDestruct (H6 with "HA") as "[HA [HC HB]]".
+           change sl2 with (nil ++ sl2).
+           iApply ("HB" with "[HA] [HC]"); eauto. 
+           change (do_set sd (Etempvar t1 ty)) with (final (For_set sd) (Etempvar t1 ty)).
+           iApply (tr_val_gen with "[HA]"). reflexivity. iIntros (? ? ? ?) "HB".
+           iDestruct ("HB"  with "HA") as "%".
+           iPureIntro. constructor. rewrite H7. apply Maps.PTree.gss.
+           iIntros (?) "HA". simpl. admit.
+    + unfold tr_top_val_val in H4. destruct sl1; auto. destruct H4 as (v'&ty0&P0&P1&P2&P3).
+      inversion P3.
 Admitted.
+
 
 (** Forward simulation for statements. *)
 
@@ -1048,8 +2315,15 @@ Lemma tr_top_val_for_val_inv:
   tr_top tge e le m For_val (Csyntax.Eval v ty) sl a -∗
   ⌜sl = nil /\ typeof a = ty /\ eval_expr tge e le m a v⌝.
 Proof.
-  Admitted.
+  iIntros (? ? ? ? ? ? ?) "HA". iDestruct "HA" as "[HA|%]".
+  - unfold tr_top_base. simpl. iDestruct "HA" as "[HA [HB [% %]]]".
+    repeat iSplit; auto. iApply "HB". eauto.
+  - unfold tr_top_val_val in H. destruct sl; auto.
+    destruct H as (v0&ty0&P0&P1&P2&P3). inversion P3. subst.
+    iPureIntro. repeat split; auto.
+Qed.
 
+    
 Lemma alloc_variables_preserved:
   forall e m params e' m',
   Csem.alloc_variables ge e m params e' m' ->
@@ -1079,13 +2353,297 @@ Qed.
 
 Lemma sstep_simulation:
   forall S1 t S2, Csem.sstep ge S1 t S2 ->
-  forall S1', match_states S1 S1' ->
-  ∃ S2',
+  forall S1' (MS: match_states S1 S1'),
+  exists S2',
      (plus step1 tge S1' t S2' \/
        (star step1 tge S1' t S2' /\ measure S2 < measure S1)%nat)
   /\ match_states S2 S2'.
 Proof.
-Admitted.
+  induction 1; intros; inv MS.
+  (* do 1 *)
+  inv H6. inv H0.
+  econstructor; split.
+  right; split. apply push_seq.
+  simpl. unfold lt. rewrite plus_n_Sm. reflexivity. 
+  econstructor; eauto. constructor. auto.
+  (* do 2 *)
+  inv H7. apply soundness3 in H6.
+  apply (soundness1 _ tmps). iIntros "HA". iDestruct (H6 with "HA") as "[[_ %]|%]".
+  iPureIntro. simpl in *; subst.
+  econstructor; split.
+  right; split. apply star_refl. simpl. unfold lt. reflexivity. 
+  econstructor; eauto. constructor.
+  unfold tr_top_val_val in H. destruct sl; auto. destruct H as (v0&ty0&P0&P1&P2&P3). inversion P2.
+  (* seq *)
+  inv H6. econstructor; split. left. apply plus_one. constructor.
+  econstructor; eauto. constructor; auto.
+(* skip seq *)
+  inv H6; inv H7. econstructor; split.
+  left. apply plus_one; constructor.
+  econstructor; eauto.
+(* continue seq *)
+  inv H6; inv H7. econstructor; split.
+  left. apply plus_one; constructor.
+  econstructor; eauto. constructor.
+(* break seq *)
+  inv H6; inv H7. econstructor; split.
+  left. apply plus_one; constructor.
+  econstructor; eauto. constructor.
+(* ifthenelse *)
+  inv H6.
+(* ifthenelse empty *)
+  inv H3. econstructor; split.
+  left. eapply plus_left. constructor. apply push_seq.
+  econstructor; eauto.
+  econstructor; eauto.
+  econstructor; eauto.
+(* ifthenelse non empty *)
+  inv H2. econstructor; split.
+  left. eapply plus_left. constructor. apply push_seq. traceEq.
+  econstructor; eauto. econstructor; eauto.
+(* ifthenelse *)
+  inv H8.
+(* ifthenelse empty *)
+  exploit tr_top_val_for_val_inv; eauto. intro. apply (soundness1 _ tmps).
+  apply soundness3 in H7. iIntros "HA". iDestruct (H7 with "HA") as "HA".
+  iDestruct (H0 with "HA") as "[% [% %]]". subst. iPureIntro.
+  econstructor; split; simpl.
+  right. destruct b; econstructor; eauto.
+  eapply star_left. apply step_skip_seq. econstructor. traceEq.
+  eapply star_left. apply step_skip_seq. econstructor. traceEq.
+  destruct b; econstructor; eauto. econstructor; eauto. econstructor; eauto.
+  (* ifthenelse non empty *)
+  exploit tr_top_val_for_val_inv; eauto. intro. apply (soundness1 _ tmps).
+  apply soundness3 in H7. iIntros "HA". iDestruct (H7 with "HA") as "HA".
+  iDestruct (H0 with "HA") as "[% [% %]]". subst. iPureIntro.
+  econstructor; split.
+  left. eapply plus_two. constructor.
+  apply step_ifthenelse with (v1 := v) (b := b); auto. traceEq.
+  destruct b; econstructor; eauto.
+(* while *)
+  inv H6. inv H1. econstructor; split.
+  left. eapply plus_left. constructor.
+  eapply star_left. constructor.
+  apply push_seq.
+  reflexivity. traceEq. rewrite Kseqlist_app.
+  econstructor; eauto. simpl.  econstructor; eauto. econstructor; eauto.
+(* while false *)
+  inv H8.
+  exploit tr_top_val_for_val_inv; eauto. intro. apply (soundness1 _ tmps).
+  apply soundness3 in H7. iIntros "HA". iDestruct (H7 with "HA") as "HA".
+  iDestruct (H0 with "HA") as "[% [% %]]". subst. iPureIntro.
+  econstructor; split.
+  left. simpl. eapply plus_left. constructor.
+  eapply star_trans. apply step_makeif with (v1 := v) (b := false); auto.
+  eapply star_two. constructor. apply step_break_loop1.
+  reflexivity. reflexivity. traceEq.
+  constructor; auto. constructor.
+(* while true *)
+  inv H8.
+  exploit tr_top_val_for_val_inv; eauto. intro. apply (soundness1 _ tmps).
+  apply soundness3 in H7. iIntros "HA". iDestruct (H7 with "HA") as "HA".
+  iDestruct (H0 with "HA") as "[% [% %]]". subst. iPureIntro. 
+  econstructor; split.
+  left. simpl. eapply plus_left. constructor.
+  eapply star_right. apply step_makeif with (v1 := v) (b := true); auto.
+  constructor.
+  reflexivity. traceEq.
+  constructor; auto. constructor; auto.
+(* skip-or-continue while *)
+  assert (ts = Sskip \/ ts = Scontinue). destruct H; subst s0; inv H7; auto.
+  inv H8.
+  econstructor; split.
+  left. eapply plus_two. apply step_skip_or_continue_loop1; auto.
+  apply step_skip_loop2. traceEq.
+  constructor; auto. constructor; auto.
+(* break while *)
+  inv H6. inv H7.
+  econstructor; split.
+  left. apply plus_one. apply step_break_loop1.
+  constructor; auto. constructor.
+
+(* dowhile *)
+  inv H6.
+  econstructor; split.
+  left. apply plus_one. apply step_loop.
+  constructor; auto. constructor; auto.
+(* skip_or_continue dowhile *)
+  assert (ts = Sskip \/ ts = Scontinue). destruct H; subst s0; inv H7; auto.
+  inv H8. inv H4.
+  econstructor; split.
+  left. eapply plus_left. apply step_skip_or_continue_loop1. auto.
+  apply push_seq.
+  traceEq.
+  rewrite Kseqlist_app.
+  econstructor; eauto. simpl. econstructor; auto. econstructor; eauto.
+(* dowhile false *)
+  inv H8.
+  exploit tr_top_val_for_val_inv; eauto. intro. apply (soundness1 _ tmps).
+  apply soundness3 in H7. iIntros "HA". iDestruct (H7 with "HA") as "HA".
+  iDestruct (H0 with "HA") as "[% [% %]]". subst. iPureIntro.
+  econstructor; split.
+  left. simpl. eapply plus_left. constructor.
+  eapply star_right. apply step_makeif with (v1 := v) (b := false); auto.
+  constructor.
+  reflexivity. traceEq.
+  constructor; auto. constructor.
+(* dowhile true *)
+  inv H8.
+  exploit tr_top_val_for_val_inv; eauto. intro. apply (soundness1 _ tmps).
+  apply soundness3 in H7. iIntros "HA". iDestruct (H7 with "HA") as "HA".
+  iDestruct (H0 with "HA") as "[% [% %]]". subst. iPureIntro.
+  econstructor; split.
+  left. simpl. eapply plus_left. constructor.
+  eapply star_right. apply step_makeif with (v1 := v) (b := true); auto.
+  constructor.
+  reflexivity. traceEq.
+  constructor; auto. constructor; auto.
+(* break dowhile *)
+  inv H6. inv H7.
+  econstructor; split.
+  left. apply plus_one. apply step_break_loop1.
+  constructor; auto. constructor.
+
+(* for start *)
+  inv H7. congruence.
+  econstructor; split.
+  left; apply plus_one. constructor.
+  econstructor; eauto. constructor; auto. econstructor; eauto.
+(* for *)
+  inv H6; try congruence. inv H2.
+  econstructor; split.
+  left. eapply plus_left. apply step_loop.
+  eapply star_left. constructor. apply push_seq.
+  reflexivity. traceEq.
+  rewrite Kseqlist_app. econstructor; eauto. simpl. constructor; auto. econstructor; eauto.
+(* for false *)
+  inv H8. exploit tr_top_val_for_val_inv; eauto. intro. apply (soundness1 _ tmps).
+  apply soundness3 in H7. iIntros "HA". iDestruct (H7 with "HA") as "HA".
+  iDestruct (H0 with "HA") as "[% [% %]]". subst. iPureIntro.
+  econstructor; split.
+  left. simpl. eapply plus_left. constructor.
+  eapply star_trans. apply step_makeif with (v1 := v) (b := false); auto.
+  eapply star_two. constructor. apply step_break_loop1.
+  reflexivity. reflexivity. traceEq.
+  constructor; auto. constructor.
+(* for true *)
+  inv H8. exploit tr_top_val_for_val_inv; eauto. intro. apply (soundness1 _ tmps).
+  apply soundness3 in H7. iIntros "HA". iDestruct (H7 with "HA") as "HA".
+  iDestruct (H0 with "HA") as "[% [% %]]". subst. iPureIntro.
+  econstructor; split.
+  left. simpl. eapply plus_left. constructor.
+  eapply star_right. apply step_makeif with (v1 := v) (b := true); auto.
+  constructor.
+  reflexivity. traceEq.
+  constructor; auto. constructor; auto.
+(* skip_or_continue for3 *)
+  assert (ts = Sskip \/ ts = Scontinue). destruct H; subst x; inv H7; auto.
+  inv H8.
+  econstructor; split.
+  left. apply plus_one. apply step_skip_or_continue_loop1. auto.
+  econstructor; eauto. econstructor; auto.
+(* break for3 *)
+  inv H6. inv H7.
+  econstructor; split.
+  left. apply plus_one. apply step_break_loop1.
+  econstructor; eauto. constructor.
+(* skip for4 *)
+  inv H6. inv H7.
+  econstructor; split.
+  left. apply plus_one. constructor.
+  econstructor; eauto. constructor; auto.
+
+
+(* return none *)
+  inv H7. econstructor; split.
+  left. apply plus_one. econstructor; eauto. rewrite blocks_of_env_preserved; eauto.
+  constructor. apply match_cont_call; auto.
+(* return some 1 *)
+  inv H6. inv H0. econstructor; split.
+  left; eapply plus_left. constructor. apply push_seq. traceEq.
+  econstructor; eauto. constructor. auto.
+(* return some 2 *)
+  inv H9. exploit tr_top_val_for_val_inv; eauto. intro. apply (soundness1 _ tmps).
+  apply soundness3 in H8. iIntros "HA". iDestruct (H8 with "HA") as "HA".
+  iDestruct (H1 with "HA") as "[% [% %]]". subst. iPureIntro.
+  econstructor; split.
+  left. eapply plus_two. constructor. econstructor. eauto.
+  erewrite function_return_preserved; eauto. rewrite blocks_of_env_preserved; eauto.
+  eauto. traceEq.
+  constructor. apply match_cont_call; auto.
+(* skip return *)
+  inv H8.
+  assert (is_call_cont tk). inv H9; simpl in *; auto.
+  econstructor; split.
+  left. apply plus_one. apply step_skip_call; eauto. rewrite blocks_of_env_preserved; eauto.
+  constructor. auto.
+  
+(* switch *)
+  inv H6. inv H1.
+  econstructor; split.
+  left; eapply plus_left. constructor. apply push_seq. traceEq.
+  econstructor; eauto. constructor; auto.
+(* expr switch *)
+  inv H8. exploit tr_top_val_for_val_inv; eauto. intro. apply (soundness1 _ tmps).
+  apply soundness3 in H7. iIntros "HA". iDestruct (H7 with "HA") as "HA".
+  iDestruct (H0 with "HA") as "[% [% %]]". subst. iPureIntro.
+  econstructor; split.
+  left; eapply plus_two. constructor. econstructor; eauto. traceEq.
+  econstructor; eauto.
+  apply tr_seq_of_labeled_statement. apply tr_select_switch. auto.
+  constructor; auto.
+
+(* skip-or-break switch *)
+  assert (ts = Sskip \/ ts = Sbreak). destruct H; subst x; inv H7; auto.
+  inv H8.
+  econstructor; split.
+  left; apply plus_one. apply step_skip_break_switch. auto.
+  constructor; auto. constructor.
+
+(* continue switch *)
+  inv H6. inv H7.
+  econstructor; split.
+  left; apply plus_one. apply step_continue_switch.
+  constructor; auto. constructor.
+
+(* label *)
+  inv H6. econstructor; split.
+  left; apply plus_one. constructor.
+  constructor; auto.
+
+(* goto *)
+  inv H7.
+  inversion H6; subst.
+  exploit tr_find_label. eauto. apply match_cont_call. eauto.
+  instantiate (1 := lbl). rewrite H.
+  intros [ts' [tk' [P [Q R]]]].
+  econstructor; split.
+  left. apply plus_one. econstructor; eauto.
+  econstructor; eauto.
+
+(* internal function *)
+  inv H7. inversion H3; subst.
+  econstructor; split.
+  left; apply plus_one. eapply step_internal_function. econstructor.
+  rewrite H6; rewrite H7; auto.
+  rewrite H6; rewrite H7. eapply alloc_variables_preserved; eauto.
+  rewrite H6. eapply bind_parameters_preserved; eauto.
+  eauto.
+  constructor; auto.
+
+(* external function *)
+  inv H5.
+  econstructor; split.
+  left; apply plus_one. econstructor; eauto.
+  eapply external_call_symbols_preserved; eauto. apply senv_preserved.
+  constructor; auto.
+
+(* return *)
+  inv H3.
+  econstructor; split.
+  left; apply plus_one. constructor.
+  econstructor; eauto.
+Qed.
 
 (** Semantic preservation *)
 
@@ -1097,55 +2655,46 @@ Theorem simulation:
        (star step1 tge S1' t S2' /\ measure S2 < measure S1)%nat)
       /\ match_states S2 S2'.
 Proof.
-Admitted.
+  intros S1 t S2 STEP. destruct STEP.
+  apply estep_simulation; auto.
+  apply sstep_simulation; auto.
+Qed.
+  
 
 Lemma transl_initial_states:
   forall S,
   Csem.initial_state prog S ->
   exists S',  Clight.initial_state tprog S' /\ match_states S S'.
 Proof.
-Admitted.
+intros. inv H.
+  exploit function_ptr_translated; eauto. intros [tf [FIND TR]].
+  econstructor; split.
+  econstructor.
+  eapply (Genv.init_mem_match (proj1 TRANSL)); eauto.
+  replace (prog_main tprog) with (prog_main prog).
+  rewrite symbols_preserved. eauto. 
+  destruct TRANSL. destruct H as (A & B & C). simpl in B. auto. 
+  eexact FIND.
+  rewrite <- H3. apply type_of_fundef_preserved. auto.
+  constructor. auto. constructor.
+Qed.
 
 Lemma transl_final_states:
   ∀ S S' r,
   match_states S S' -> Csem.final_state S r -> Clight.final_state S' r.
 Proof.
-Admitted.
-
-Lemma test : forall (P : iProp) Q tmps, Q /\ P () tmps <-> (\⌜Q⌝ ∗ P) () tmps.
-Proof.
-  intros.
-  split; intro.
-  - destruct H. apply soundness2. apply soundness3 in H0. iIntros "HA".
-    iDestruct (H0 with "HA") as "HA". iFrame. iPureIntro. apply H.
-  - apply soundness3 in H. split.
-    + apply (soundness1 _ tmps). iIntros "HA". iDestruct (H with "HA") as "[HA HB]". iFrame.
-    + apply soundness2. iIntros "HA". iDestruct (H with "HA") as "[HA HB]". iFrame.
+  intros. inv H0. inv H. inv H4. constructor.
 Qed.
-
-Print forward_simulation_star_wf.
 
 Theorem transl_program_correct:
   forward_simulation (Cstrategy.semantics prog) (Clight.semantics1 tprog).
 Proof.
-  Locate forward_simulation_star_wf.
-  Print forward_simulation. Print fsim_properties.
-  Print forward_simulation_star_wf.
   eapply forward_simulation_star_wf with (order := ltof _ measure).
   eapply senv_preserved.
-  - intros. eapply transl_initial_states in H. destruct H as (S'&P0&P1).
-    exists S'. split; auto. eapply P1.
-  - simpl. intros.
-    eapply transl_final_states; eauto. 
-  - apply well_founded_ltof.
-  - simpl. intros. eapply simulation in H. instantiate (1 := s2) in H.
-    instantiate (1 := ∅).
-    apply soundness3 in H0. eapply (soundness1 _ ∅).
-    iIntros "HA". iDestruct (H0 with "HA") as "HA".
-    iDestruct (H with "HA") as (s2') "[% HA]".
-    pose init_heap. apply H0 in b.
-
-    exact simulation.
+  eexact transl_initial_states.
+  eexact transl_final_states.
+  apply well_founded_ltof.
+  exact simulation.
 Qed.
 
 End PRESERVATION.
